more

thys/POPLmark/Pattern.thy
@@ -2,23 +2,23 @@ theory Pattern
   imports POPLmark_1B
 begin
 
-datatype ('tv::var, PPVars: 'v) prepat = PPVar 'v "'tv typ" | PPRec "(label, ('tv, 'v) prepat) lfset"
+datatype ('tvar::var, PPV: 'var) ppat = PPVr 'var "'tvar type" | PPRec "(label, ('tvar, 'var) ppat) lfset"
 
-lemma finite_PPVars: "finite (PPVars P)"
+lemma finite_PPV: "finite (PPV P)"
   by (induct P) auto
 
-definition nonrep_prepat :: "('tv::var, 'v::var) prepat \<Rightarrow> bool" where
-  "nonrep_prepat P = (\<forall>Q :: ('tv, 'v) prepat. rel_prepat top P Q \<longrightarrow> (\<exists>f. Q = map_prepat f P))"
+definition nonrep_ppat :: "('tv::var, 'v::var) ppat \<Rightarrow> bool" where
+  "nonrep_ppat P = (\<forall>Q :: ('tv, 'v) ppat. rel_ppat top P Q \<longrightarrow> (\<exists>f. Q = map_ppat f P))"
 
-lemma nonrep_prepat_PPVar[simp]: "nonrep_prepat (PPVar x T)"
-  unfolding nonrep_prepat_def
+lemma nonrep_ppat_PPVar[simp]: "nonrep_ppat (PPVr x T)"
+  unfolding nonrep_ppat_def
   apply safe
   subgoal for Q
     by (cases Q; auto)
   done
 
-lemma PVars_bd: "|PPVars (x :: ('tv::var, 'v::var) prepat)| <o |UNIV :: 'v::var set|"
-  by (rule ordLess_ordLeq_trans[OF prepat.set_bd]) (simp add: typ_pre.var_large)
+lemma PV_bd: "|PPV (x :: ('tv::var, 'v::var) ppat)| <o |UNIV :: 'v::var set|"
+  by (rule ordLess_ordLeq_trans[OF ppat.set_bd]) (simp add: type_pre.var_large)
 
 lemma values_lfupdate: "values (lfupdate X y x) \<subseteq> insert x (values X)"
   including lfset.lifting
@@ -36,25 +36,25 @@ lemma lfin_lfupdate: "(x, Q) \<in>\<in> X\<lbrace>y := T\<rbrace> \<longleftrigh
   including lfset.lifting
   by transfer auto
 
-lemma map_prepat_idleD: "map_prepat f P = P \<Longrightarrow> z \<in> PPVars P \<Longrightarrow> f z = z"
+lemma map_ppat_idleD: "map_ppat f P = P \<Longrightarrow> z \<in> PPV P \<Longrightarrow> f z = z"
   apply (induct P)
    apply auto
   by (metis lfin_label_inject lfin_map_lfset values_lfin)
 
-lemma map_prepat_swapD: "map_prepat f Q = map_prepat (id(z := z', z' := z)) Q \<Longrightarrow> z \<in> PPVars Q \<Longrightarrow> f z = z'"
+lemma map_ppat_swapD: "map_ppat f Q = map_ppat (id(z := z', z' := z)) Q \<Longrightarrow> z \<in> PPV Q \<Longrightarrow> f z = z'"
   apply (induct Q)
    apply auto
   by (metis (no_types, opaque_lifting) lfin_label_inject lfin_map_lfset values_lfin)
 
-lemma nonrep_prepat_PRecD1: "nonrep_prepat (PPRec X :: ('tv::var, 'v::var) prepat) \<Longrightarrow> (x, P) \<in>\<in> X \<Longrightarrow>
-  nonrep_prepat P"
-  unfolding nonrep_prepat_def
+lemma nonrep_ppat_PRecD1: "nonrep_ppat (PPRec X :: ('tv::var, 'v::var) ppat) \<Longrightarrow> (x, P) \<in>\<in> X \<Longrightarrow>
+  nonrep_ppat P"
+  unfolding nonrep_ppat_def
   apply safe
   subgoal for Q
     apply (drule spec[where x="PPRec (X\<lbrace>x := Q\<rbrace>)"])
     apply (drule mp)
      apply (auto simp: lfset.in_rel[of id, simplified, unfolded lfset.map_id]
-      map_lfset_lfupdate lfset.set_map lfset.map_comp o_def lfset.map_ident prepat.rel_refl lfupdate_idle
+      map_lfset_lfupdate lfset.set_map lfset.map_comp o_def lfset.map_ident ppat.rel_refl lfupdate_idle
       dest!: set_mp[OF values_lfupdate]
        intro!: exI[of _ "lfupdate (map_lfset id (\<lambda>P. (P, P)) X) x (P, Q)"]) []
     apply (erule exE)
@@ -65,94 +65,94 @@ lemma nonrep_prepat_PRecD1: "nonrep_prepat (PPRec X :: ('tv::var, 'v::var) prepa
     done
   done
 
-lemma nonrep_prepat_PRecD2: "nonrep_prepat (PPRec X :: ('tv::var, 'v::var) prepat) \<Longrightarrow>
-  (\<forall>x y P Q. x \<noteq> y \<longrightarrow> (x, P) \<in>\<in> X \<longrightarrow> (y, Q) \<in>\<in> X \<longrightarrow> PPVars P \<inter> PPVars Q = {})"
-proof (unfold nonrep_prepat_def, safe, goal_cases LR)
+lemma nonrep_ppat_PRecD2: "nonrep_ppat (PPRec X :: ('tv::var, 'v::var) ppat) \<Longrightarrow>
+  (\<forall>x y P Q. x \<noteq> y \<longrightarrow> (x, P) \<in>\<in> X \<longrightarrow> (y, Q) \<in>\<in> X \<longrightarrow> PPV P \<inter> PPV Q = {})"
+proof (unfold nonrep_ppat_def, safe, goal_cases LR)
   case (LR x y P Q z)
-  obtain z' where "z' \<notin> PPVars (PPRec X)"
-    using MRBNF_FP.exists_fresh[OF PVars_bd] by blast
-  with LR(4) have "rel_prepat top (PPRec X) (PPRec (lfupdate X y (map_prepat (id(z := z', z' := z)) Q)))"
+  obtain z' where "z' \<notin> PPV (PPRec X)"
+    using MRBNF_FP.exists_fresh[OF PV_bd] by blast
+  with LR(4) have "rel_ppat top (PPRec X) (PPRec (lfupdate X y (map_ppat (id(z := z', z' := z)) Q)))"
     by (auto simp: lfset.in_rel[of id, simplified, unfolded lfset.map_id]
       map_lfset_lfupdate lfset.map_comp o_def lfset.map_ident
-      prepat.rel_map prepat.rel_refl lfset.set_map lfupdate_idle
+      ppat.rel_map ppat.rel_refl lfset.set_map lfupdate_idle
       dest!: set_mp[OF values_lfupdate]
-      intro!: exI[of _ "lfupdate (map_lfset id (\<lambda>P. (P, P)) X) y (Q, map_prepat (id(z := z', z' := z)) Q)"])
-  with LR(1) obtain f where "map_prepat f (PPRec X) = PPRec (lfupdate X y (map_prepat (id(z := z', z' := z)) Q))"
+      intro!: exI[of _ "lfupdate (map_lfset id (\<lambda>P. (P, P)) X) y (Q, map_ppat (id(z := z', z' := z)) Q)"])
+  with LR(1) obtain f where "map_ppat f (PPRec X) = PPRec (lfupdate X y (map_ppat (id(z := z', z' := z)) Q))"
     by metis
-  then have *: "map_lfset id (map_prepat f) X = X\<lbrace>y := map_prepat (id(z := z', z' := z)) Q\<rbrace>"
-    by (auto dest!: arg_cong[where f=PPVars])
-  then have "map_prepat f P = P"
-    using LR(2) lfin_map_lfset[THEN iffD2, OF exI, OF conjI, OF _ LR(3), of "map_prepat f P" "map_prepat f"]
+  then have *: "map_lfset id (map_ppat f) X = X\<lbrace>y := map_ppat (id(z := z', z' := z)) Q\<rbrace>"
+    by (auto dest!: arg_cong[where f=PPV])
+  then have "map_ppat f P = P"
+    using LR(2) lfin_map_lfset[THEN iffD2, OF exI, OF conjI, OF _ LR(3), of "map_ppat f P" "map_ppat f"]
     by (auto simp: lfin_lfupdate lfin_label_inject LR(3))
   then have "f z = z"
-    using LR(5) map_prepat_idleD by metis
-  moreover from * have "map_prepat f Q = map_prepat (id(z := z', z' := z)) Q"
-    using lfin_map_lfset[THEN iffD2, OF exI, OF conjI, OF _ LR(4), of "map_prepat f Q" "map_prepat f"]
+    using LR(5) map_ppat_idleD by metis
+  moreover from * have "map_ppat f Q = map_ppat (id(z := z', z' := z)) Q"
+    using lfin_map_lfset[THEN iffD2, OF exI, OF conjI, OF _ LR(4), of "map_ppat f Q" "map_ppat f"]
     by (auto simp: lfin_lfupdate)
   then have "f z = z'"
-    using LR(6) map_prepat_swapD by metis
+    using LR(6) map_ppat_swapD by metis
   ultimately show ?case
-    by (metis LR(3,5) \<open>z' \<notin> PPVars (PPRec X)\<close> lfin_values prepat.set_intros(2))
+    by (metis LR(3,5) \<open>z' \<notin> PPV (PPRec X)\<close> lfin_values ppat.set_intros(2))
 qed
 
 lemma lfset_eq_iff: "X = Y \<longleftrightarrow> (\<forall>x P. (x, P) \<in>\<in> X \<longleftrightarrow> (x, P) \<in>\<in> Y)"
   including lfset.lifting
   by transfer auto
 
-lemma nonrep_prepat_PRecI:
+lemma nonrep_ppat_PRecI:
   assumes
-    "(\<forall>x P. (x, P) \<in>\<in> X \<longrightarrow> nonrep_prepat P)"
-    "(\<forall>x y P Q. x \<noteq> y \<longrightarrow> (x, P) \<in>\<in> X \<longrightarrow> (y, Q) \<in>\<in> X \<longrightarrow> PPVars P \<inter> PPVars Q = {})"
-  shows "nonrep_prepat (PPRec X :: ('tv::var, 'v::var) prepat)"
+    "(\<forall>x P. (x, P) \<in>\<in> X \<longrightarrow> nonrep_ppat P)"
+    "(\<forall>x y P Q. x \<noteq> y \<longrightarrow> (x, P) \<in>\<in> X \<longrightarrow> (y, Q) \<in>\<in> X \<longrightarrow> PPV P \<inter> PPV Q = {})"
+  shows "nonrep_ppat (PPRec X :: ('tv::var, 'v::var) ppat)"
   using assms
-  unfolding nonrep_prepat_def
+  unfolding nonrep_ppat_def
 proof (safe, goal_cases RL)
   case (RL QQ)
   then obtain Y where "QQ = PPRec Y"
     by (cases QQ; simp)
-  with RL(3) have *: "rel_lfset id (rel_prepat top) X Y" by auto
+  with RL(3) have *: "rel_lfset id (rel_ppat top) X Y" by auto
   { fix x P
     assume xP: "(x, P) \<in>\<in> X"
-    with * obtain Q where "(x, Q) \<in>\<in> Y" "rel_prepat top P Q"
+    with * obtain Q where "(x, Q) \<in>\<in> Y" "rel_ppat top P Q"
       including lfset.lifting
       by (atomize_elim, transfer) (force simp: rel_fset_alt)
     moreover
-    from assms(1) xP \<open>rel_prepat top P Q\<close> obtain f where "map_prepat f P = Q"
-      unfolding nonrep_prepat_def by blast
-    then obtain g where "supp g \<subseteq> PPVars P" "map_prepat g P = Q"
-      by (atomize_elim, intro exI[of _ "\<lambda>x. if x \<in> PPVars P then f x else x"])
-        (auto simp: supp_def intro: prepat.map_cong)
-    ultimately have "\<exists>f. (x, map_prepat f P) \<in>\<in> Y \<and> supp f \<subseteq> PPVars P"
+    from assms(1) xP \<open>rel_ppat top P Q\<close> obtain f where "map_ppat f P = Q"
+      unfolding nonrep_ppat_def by blast
+    then obtain g where "supp g \<subseteq> PPV P" "map_ppat g P = Q"
+      by (atomize_elim, intro exI[of _ "\<lambda>x. if x \<in> PPV P then f x else x"])
+        (auto simp: supp_def intro: ppat.map_cong)
+    ultimately have "\<exists>f. (x, map_ppat f P) \<in>\<in> Y \<and> supp f \<subseteq> PPV P"
       by auto
   } note pick_ex = this
-  define pick where "pick = (\<lambda>x (P :: ('tv::var, 'v::var) prepat). SOME f. (x, map_prepat f P) \<in>\<in> Y \<and> supp f \<subseteq> PPVars P)"
-  have pick: "(x, map_prepat (pick x P) P) \<in>\<in> Y" "supp (pick x P) \<subseteq> PPVars P" if "(x, P) \<in>\<in> X" for x P
+  define pick where "pick = (\<lambda>x (P :: ('tv::var, 'v::var) ppat). SOME f. (x, map_ppat f P) \<in>\<in> Y \<and> supp f \<subseteq> PPV P)"
+  have pick: "(x, map_ppat (pick x P) P) \<in>\<in> Y" "supp (pick x P) \<subseteq> PPV P" if "(x, P) \<in>\<in> X" for x P
     using someI_ex[OF pick_ex[OF that]] unfolding pick_def
     by (auto simp: Eps_case_prod)
-  define pick_part where "pick_part = (\<lambda>z. THE (x, P). (x, P) \<in>\<in> X \<and> z \<in> PPVars P)"
-  have pick_part: "pick_part z \<in>\<in> X \<and> z \<in> PPVars (snd (pick_part z))" if "\<exists>x P. (x, P) \<in>\<in> X \<and> z \<in> PPVars P" for z
+  define pick_part where "pick_part = (\<lambda>z. THE (x, P). (x, P) \<in>\<in> X \<and> z \<in> PPV P)"
+  have pick_part: "pick_part z \<in>\<in> X \<and> z \<in> PPV (snd (pick_part z))" if "\<exists>x P. (x, P) \<in>\<in> X \<and> z \<in> PPV P" for z
     using that assms(2) unfolding pick_part_def
     apply -
     apply (rule the1I2)
      apply auto
      apply blast
     by (metis Int_emptyD lfin_label_inject)
-  define pick1 where "pick1 = (\<lambda>z. if \<exists>x P. (x, P) \<in>\<in> X \<and> z \<in> PPVars P then case_prod pick (pick_part z) z else z)"
+  define pick1 where "pick1 = (\<lambda>z. if \<exists>x P. (x, P) \<in>\<in> X \<and> z \<in> PPV P then case_prod pick (pick_part z) z else z)"
   show ?case
     unfolding \<open>QQ = PPRec Y\<close>
     apply (auto intro!: exI[of _ pick1] simp: pick1_def lfset_eq_iff lfin_map_lfset)
     subgoal for x P
-      apply (subgoal_tac "\<exists>P'. (x, P') \<in>\<in> X \<and> rel_prepat top P' P")
+      apply (subgoal_tac "\<exists>P'. (x, P') \<in>\<in> X \<and> rel_ppat top P' P")
        apply auto
        apply (frule pick)
       subgoal for P'
         apply (rule exI[of _ P'])
         apply auto
         apply (rule sym)
-        apply (rule trans[OF prepat.map_cong[OF refl]])
+        apply (rule trans[OF ppat.map_cong[OF refl]])
          apply (rule if_P)
          apply (auto simp: split_beta)
-        apply (rule trans[OF prepat.map_cong[OF refl], of _ _ "pick x P'"])
+        apply (rule trans[OF ppat.map_cong[OF refl], of _ _ "pick x P'"])
         apply (metis Int_emptyD assms(2) lfin_label_inject pick_part surjective_pairing)
         apply (simp add: lfin_label_inject)
         done
@@ -164,31 +164,31 @@ proof (safe, goal_cases RL)
     subgoal for x P
       apply (frule pick)
       using
-        \<open>\<And>x P. (x, P) \<in>\<in> Y \<Longrightarrow> \<exists>c. P = map_prepat (\<lambda>z. if \<exists>x P. (x, P) \<in>\<in> X \<and> z \<in> PPVars P then (case pick_part z of (x, xa) \<Rightarrow> pick x xa) z else z) c \<and> (x, c) \<in>\<in> X\<close>
+        \<open>\<And>x P. (x, P) \<in>\<in> Y \<Longrightarrow> \<exists>c. P = map_ppat (\<lambda>z. if \<exists>x P. (x, P) \<in>\<in> X \<and> z \<in> PPV P then (case pick_part z of (x, xa) \<Rightarrow> pick x xa) z else z) c \<and> (x, c) \<in>\<in> X\<close>
         lfin_label_inject by fastforce
     done
 qed
 
-definition "nonrep_PPRec X = (\<forall>x y P Q. x \<noteq> y \<longrightarrow> (x, P) \<in>\<in> X \<longrightarrow> (y, Q) \<in>\<in> X \<longrightarrow> PPVars P \<inter> PPVars Q = {})"
+definition "nonrep_PPRec X = (\<forall>x y P Q. x \<noteq> y \<longrightarrow> (x, P) \<in>\<in> X \<longrightarrow> (y, Q) \<in>\<in> X \<longrightarrow> PPV P \<inter> PPV Q = {})"
 
 lemma nonrep_PPRec_lfemtpy[simp]: "nonrep_PPRec lfempty"
   unfolding nonrep_PPRec_def by auto
 
-lemma nonrep_prepat_PRec[simp]: "nonrep_prepat (PPRec X :: ('tv::var, 'v::var) prepat) \<longleftrightarrow>
-  ((\<forall>x P. (x, P) \<in>\<in> X \<longrightarrow> nonrep_prepat P) \<and>
+lemma nonrep_ppat_PRec[simp]: "nonrep_ppat (PPRec X :: ('tv::var, 'v::var) ppat) \<longleftrightarrow>
+  ((\<forall>x P. (x, P) \<in>\<in> X \<longrightarrow> nonrep_ppat P) \<and>
   nonrep_PPRec X)"
   unfolding nonrep_PPRec_def
-  using nonrep_prepat_PRecI[of X] nonrep_prepat_PRecD1[of X] nonrep_prepat_PRecD2[of X] by blast
+  using nonrep_ppat_PRecI[of X] nonrep_ppat_PRecD1[of X] nonrep_ppat_PRecD2[of X] by blast
 
-typedef ('tv::var, 'v::var) pat = "{p :: ('tv, 'v) prepat. nonrep_prepat p}"
-  by (auto intro!: exI[of _ "PPVar undefined undefined"])
+typedef ('tv::var, 'v::var) pat = "{p :: ('tv, 'v) ppat. nonrep_ppat p}"
+  by (auto intro!: exI[of _ "PPVr undefined undefined"])
 
 setup_lifting type_definition_pat
 
-lift_definition PVar :: "'v \<Rightarrow> 'tv typ \<Rightarrow> ('tv::var, 'v::var) pat" is PPVar
+lift_definition PVr :: "'v \<Rightarrow> 'tv type \<Rightarrow> ('tv::var, 'v::var) pat" is PPVr
   by auto
 
-lemma PVar_inject[simp]: "PVar X T = PVar Y U \<longleftrightarrow> X = Y \<and> T = U"
+lemma PVar_inject[simp]: "PVr X T = PVr Y U \<longleftrightarrow> X = Y \<and> T = U"
   by transfer auto
 
 definition PRec :: "(label, ('tv::var, 'v::var) pat) lfset \<Rightarrow> ('tv::var, 'v::var) pat" where
@@ -204,132 +204,132 @@ lemma PRec_transfer[transfer_rule]: "rel_fun (rel_lfset id cr_pat) cr_pat (\<lam
   apply (simp_all add: lfset.map_cong_id)
   done
 
-fun vvsubst_prepat where
-  "vvsubst_prepat \<tau> \<sigma> (PPVar v T) = PPVar (\<sigma> v) (vvsubst_typ \<tau> T)"
-| "vvsubst_prepat \<tau> \<sigma> (PPRec X) = PPRec (map_lfset id (vvsubst_prepat \<tau> \<sigma>) X)"
+fun vvsubst_ppat where
+  "vvsubst_ppat \<tau> \<sigma> (PPVr v T) = PPVr (\<sigma> v) (vvsubst_type \<tau> T)"
+| "vvsubst_ppat \<tau> \<sigma> (PPRec X) = PPRec (map_lfset id (vvsubst_ppat \<tau> \<sigma>) X)"
 
-fun tvsubst_prepat where
-  "tvsubst_prepat \<tau> \<sigma> (PPVar v T) = PPVar (\<sigma> v) (tvsubst_typ \<tau> T)"
-| "tvsubst_prepat \<tau> \<sigma> (PPRec X) = PPRec (map_lfset id (tvsubst_prepat \<tau> \<sigma>) X)"
+fun subst_ppat where
+  "subst_ppat \<tau> \<sigma> (PPVr v T) = PPVr (\<sigma> v) (substT \<tau> T)"
+| "subst_ppat \<tau> \<sigma> (PPRec X) = PPRec (map_lfset id (subst_ppat \<tau> \<sigma>) X)"
 
-fun PPTVars where
-  "PPTVars (PPVar v T) = FVars_typ T"
-| "PPTVars (PPRec X) = (\<Union>P \<in> values X. PPTVars P)"
+fun PPTV where
+  "PPTV (PPVr v T) = TFV T"
+| "PPTV (PPRec X) = (\<Union>P \<in> values X. PPTV P)"
 
-lemma finite_PPTVars: "finite (PPTVars P)"
+lemma finite_PPTV: "finite (PPTV P)"
   by (induct P) auto
 
-lemma PPVars_vvsubst_prepat[simp]: "PPVars (vvsubst_prepat \<tau> \<sigma> P) = \<sigma> ` PPVars P"
+lemma PPV_vvsubst_ppat[simp]: "PPV (vvsubst_ppat \<tau> \<sigma> P) = \<sigma> ` PPV P"
   by (induct P) (auto simp: lfset.set_map)
 
-lemma PPVars_tvsubst_prepat[simp]: "PPVars (tvsubst_prepat \<tau> \<sigma> P) = \<sigma> ` PPVars P"
+lemma PPV_subst_ppat[simp]: "PPV (subst_ppat \<tau> \<sigma> P) = \<sigma> ` PPV P"
   by (induct P) (auto simp: lfset.set_map)
 
-lemma PPTVars_vvsubst_prepat[simp]:
-  fixes P :: "('tv::var, 'v::var) prepat"
-  shows "|supp \<tau>| <o |UNIV :: 'tv::var set| \<Longrightarrow> PPTVars (vvsubst_prepat \<tau> \<sigma> P) = \<tau> ` PPTVars P"
-  by (induct P) (auto simp: lfset.set_map typ.set_map)
+lemma PPTV_vvsubst_ppat[simp]:
+  fixes P :: "('tv::var, 'v::var) ppat"
+  shows "|supp \<tau>| <o |UNIV :: 'tv::var set| \<Longrightarrow> PPTV (vvsubst_ppat \<tau> \<sigma> P) = \<tau> ` PPTV P"
+  by (induct P) (auto simp: lfset.set_map type.set_map)
 
-lemma PPTVars_tvsubst_prepat[simp]: 
-  fixes P :: "('tv::var, 'v::var) prepat"
-  shows "|SSupp_typ \<tau>| <o |UNIV :: 'tv::var set| \<Longrightarrow> PPTVars (tvsubst_prepat \<tau> \<sigma> P) = (\<Union>x \<in> PPTVars P. FVars_typ (\<tau> x))"
-  by (induct P) (auto simp: lfset.set_map FVars_tvsubst_typ)
+lemma PPTV_subst_ppat[simp]: 
+  fixes P :: "('tv::var, 'v::var) ppat"
+  shows "|SSupp_type \<tau>| <o |UNIV :: 'tv::var set| \<Longrightarrow> PPTV (subst_ppat \<tau> \<sigma> P) = (\<Union>x \<in> PPTV P. TFV (\<tau> x))"
+  by (induct P) (auto simp: lfset.set_map FVars_substT)
 
-lemma nonrep_prepat_vvsubst_prepat:
-  "bij \<sigma> \<Longrightarrow> nonrep_prepat P \<Longrightarrow> nonrep_prepat (vvsubst_prepat \<tau> \<sigma> P)"
+lemma nonrep_ppat_vvsubst_ppat:
+  "bij \<sigma> \<Longrightarrow> nonrep_ppat P \<Longrightarrow> nonrep_ppat (vvsubst_ppat \<tau> \<sigma> P)"
   apply (induct P)
    apply (auto simp: lfin_map_lfset lfin_values nonrep_PPRec_def)
   apply (metis Int_emptyD bij_implies_inject)
   done
 
 lift_definition vvsubst_pat :: "('tv \<Rightarrow> 'tv) \<Rightarrow> ('v \<Rightarrow> 'v) \<Rightarrow> ('tv::var, 'v::var) pat \<Rightarrow> ('tv::var, 'v::var) pat" is
-  "\<lambda>\<tau> \<sigma>. if bij \<sigma> then vvsubst_prepat \<tau> \<sigma> else id"
-  by (auto simp: nonrep_prepat_vvsubst_prepat)
+  "\<lambda>\<tau> \<sigma>. if bij \<sigma> then vvsubst_ppat \<tau> \<sigma> else id"
+  by (auto simp: nonrep_ppat_vvsubst_ppat)
 
-lemma nonrep_prepat_tvsubst_prepat:
-  "bij \<sigma> \<Longrightarrow> nonrep_prepat P \<Longrightarrow> nonrep_prepat (tvsubst_prepat \<tau> \<sigma> P)"
+lemma nonrep_ppat_subst_ppat:
+  "bij \<sigma> \<Longrightarrow> nonrep_ppat P \<Longrightarrow> nonrep_ppat (subst_ppat \<tau> \<sigma> P)"
   apply (induct P)
    apply (auto simp: lfin_map_lfset lfin_values nonrep_PPRec_def)
   apply (metis Int_emptyD bij_implies_inject)
   done
 
-lift_definition tvsubst_pat :: "('tv \<Rightarrow> 'tv typ) \<Rightarrow> ('v \<Rightarrow> 'v) \<Rightarrow> ('tv::var, 'v::var) pat \<Rightarrow> ('tv::var, 'v::var) pat" is
-  "\<lambda>\<tau> \<sigma>. if bij \<sigma> then tvsubst_prepat \<tau> \<sigma> else id"
-  by (auto simp: nonrep_prepat_tvsubst_prepat)
+lift_definition subst_pat :: "('tv \<Rightarrow> 'tv type) \<Rightarrow> ('v \<Rightarrow> 'v) \<Rightarrow> ('tv::var, 'v::var) pat \<Rightarrow> ('tv::var, 'v::var) pat" is
+  "\<lambda>\<tau> \<sigma>. if bij \<sigma> then subst_ppat \<tau> \<sigma> else id"
+  by (auto simp: nonrep_ppat_subst_ppat)
 
-lift_definition PVars :: "('tv::var, 'v::var) pat \<Rightarrow> 'v set" is
-  "PPVars" .
+lift_definition PV :: "('tv::var, 'v::var) pat \<Rightarrow> 'v set" is
+  "PPV" .
 
-lift_definition PTVars :: "('tv::var, 'v::var) pat \<Rightarrow> 'tv set" is
-  "PPTVars" .
+lift_definition PTV :: "('tv::var, 'v::var) pat \<Rightarrow> 'tv set" is
+  "PPTV" .
 
-lemma PVars_vvsubst_pat: "bij \<sigma> \<Longrightarrow> PVars (vvsubst_pat \<tau> \<sigma> P) = \<sigma> ` PVars P"
+lemma PV_vvsubst_pat: "bij \<sigma> \<Longrightarrow> PV (vvsubst_pat \<tau> \<sigma> P) = \<sigma> ` PV P"
   by transfer auto
 
-lemma PVars_tvsubst_pat: "bij \<sigma> \<Longrightarrow> PVars (tvsubst_pat \<tau> \<sigma> P) = \<sigma> ` PVars P"
+lemma PV_subst_pat: "bij \<sigma> \<Longrightarrow> PV (subst_pat \<tau> \<sigma> P) = \<sigma> ` PV P"
   by transfer auto
 
-lemma PTVars_vvsubst_pat:
+lemma PTV_vvsubst_pat:
   fixes P :: "('tv::var, 'v::var) pat"
-  shows "|supp \<tau>| <o |UNIV :: 'tv::var set| \<Longrightarrow> bij \<sigma> \<Longrightarrow> PTVars (vvsubst_pat \<tau> \<sigma> P) = \<tau> ` PTVars P"
+  shows "|supp \<tau>| <o |UNIV :: 'tv::var set| \<Longrightarrow> bij \<sigma> \<Longrightarrow> PTV (vvsubst_pat \<tau> \<sigma> P) = \<tau> ` PTV P"
   by transfer auto
 
-lemma PTVars_tvsubst_pat:
+lemma PTV_subst_pat:
   fixes P :: "('tv::var, 'v::var) pat"
-  shows "|SSupp_typ \<tau>| <o |UNIV :: 'tv::var set| \<Longrightarrow> bij \<sigma> \<Longrightarrow> PTVars (tvsubst_pat \<tau> \<sigma> P) = (\<Union>x \<in> PTVars P. FVars_typ (\<tau> x))"
+  shows "|SSupp_type \<tau>| <o |UNIV :: 'tv::var set| \<Longrightarrow> bij \<sigma> \<Longrightarrow> PTV (subst_pat \<tau> \<sigma> P) = (\<Union>x \<in> PTV P. TFV (\<tau> x))"
   by transfer auto
 
-lemma vvsubst_prepat_tvsubst_prepat:
-  fixes P :: "('tv::var, 'v::var) prepat"
+lemma vvsubst_ppat_subst_ppat:
+  fixes P :: "('tv::var, 'v::var) ppat"
   shows "|supp \<tau>| <o |UNIV :: 'tv::var set| \<Longrightarrow>
-    vvsubst_prepat \<tau> \<sigma> P = tvsubst_prepat (TyVar o \<tau>) \<sigma> P"
-  by (induct P) (auto simp: vvsubst_typ_tvsubst_typ intro!: lfset.map_cong)
+    vvsubst_ppat \<tau> \<sigma> P = subst_ppat (TVr o \<tau>) \<sigma> P"
+  by (induct P) (auto simp: vvsubst_type_substT intro!: lfset.map_cong)
 
-lemma vvsubst_pat_tvsubst_pat:
+lemma vvsubst_pat_subst_pat:
   fixes P :: "('tv::var, 'v::var) pat"
   shows "|supp \<tau>| <o |UNIV :: 'tv::var set| \<Longrightarrow>
-    vvsubst_pat \<tau> \<sigma> P = tvsubst_pat (TyVar o \<tau>) \<sigma> P"
-  by transfer (auto simp: vvsubst_prepat_tvsubst_prepat)
+    vvsubst_pat \<tau> \<sigma> P = subst_pat (TVr o \<tau>) \<sigma> P"
+  by transfer (auto simp: vvsubst_ppat_subst_ppat)
 
-lemma tvsubst_prepat_comp:
-  fixes P :: "('tv::var, 'v::var) prepat"
-  shows "|SSupp_typ \<tau>| <o |UNIV :: 'tv::var set| \<Longrightarrow> |SSupp_typ \<tau>'| <o |UNIV :: 'tv::var set| \<Longrightarrow>
-    tvsubst_prepat \<tau> \<sigma> (tvsubst_prepat \<tau>' \<sigma>' P) = tvsubst_prepat (tvsubst_typ \<tau> o \<tau>') (\<sigma> o \<sigma>') P"
-  by (induct P) (auto simp: tvsubst_typ_comp lfset.map_comp intro!: lfset.map_cong)
+lemma subst_ppat_comp:
+  fixes P :: "('tv::var, 'v::var) ppat"
+  shows "|SSupp_type \<tau>| <o |UNIV :: 'tv::var set| \<Longrightarrow> |SSupp_type \<tau>'| <o |UNIV :: 'tv::var set| \<Longrightarrow>
+    subst_ppat \<tau> \<sigma> (subst_ppat \<tau>' \<sigma>' P) = subst_ppat (substT \<tau> o \<tau>') (\<sigma> o \<sigma>') P"
+  by (induct P) (auto simp: substT_comp lfset.map_comp intro!: lfset.map_cong)
 
-lemma tvsubst_prepat_cong:
-  fixes P :: "('tv::var, 'v::var) prepat"
-  shows "|SSupp_typ \<tau>| <o |UNIV :: 'tv::var set| \<Longrightarrow> |SSupp_typ \<tau>'| <o |UNIV :: 'tv::var set| \<Longrightarrow>
-  (\<forall>x \<in> PPTVars P. \<tau> x = \<tau>' x) \<Longrightarrow> (\<forall>x \<in> PPVars P. \<sigma> x = \<sigma>' x) \<Longrightarrow>  
-  tvsubst_prepat \<tau> \<sigma> P = tvsubst_prepat \<tau>' \<sigma>' P"
-  by (induct P) (auto intro!: lfset.map_cong tvsubst_typ_cong)
+lemma subst_ppat_cong:
+  fixes P :: "('tv::var, 'v::var) ppat"
+  shows "|SSupp_type \<tau>| <o |UNIV :: 'tv::var set| \<Longrightarrow> |SSupp_type \<tau>'| <o |UNIV :: 'tv::var set| \<Longrightarrow>
+  (\<forall>x \<in> PPTV P. \<tau> x = \<tau>' x) \<Longrightarrow> (\<forall>x \<in> PPV P. \<sigma> x = \<sigma>' x) \<Longrightarrow>  
+  subst_ppat \<tau> \<sigma> P = subst_ppat \<tau>' \<sigma>' P"
+  by (induct P) (auto intro!: lfset.map_cong substT_cong)
 
-lemma tvsubst_pat_comp:
+lemma subst_pat_comp:
   fixes P :: "('tv::var, 'v::var) pat"
-  shows "|SSupp_typ \<tau>| <o |UNIV :: 'tv::var set| \<Longrightarrow> |SSupp_typ \<tau>'| <o |UNIV :: 'tv::var set| \<Longrightarrow> bij \<sigma> \<Longrightarrow> bij \<sigma>' \<Longrightarrow>
-    tvsubst_pat \<tau> \<sigma> (tvsubst_pat \<tau>' \<sigma>' P) = tvsubst_pat (tvsubst_typ \<tau> o \<tau>') (\<sigma> o \<sigma>') P"
-  by transfer (auto simp: tvsubst_prepat_comp)
+  shows "|SSupp_type \<tau>| <o |UNIV :: 'tv::var set| \<Longrightarrow> |SSupp_type \<tau>'| <o |UNIV :: 'tv::var set| \<Longrightarrow> bij \<sigma> \<Longrightarrow> bij \<sigma>' \<Longrightarrow>
+    subst_pat \<tau> \<sigma> (subst_pat \<tau>' \<sigma>' P) = subst_pat (substT \<tau> o \<tau>') (\<sigma> o \<sigma>') P"
+  by transfer (auto simp: subst_ppat_comp)
 
-lemma tvsubst_pat_cong:
+lemma subst_pat_cong:
   fixes P :: "('tv::var, 'v::var) pat"
-  shows "|SSupp_typ \<tau>| <o |UNIV :: 'tv::var set| \<Longrightarrow> |SSupp_typ \<tau>'| <o |UNIV :: 'tv::var set| \<Longrightarrow> bij \<sigma> \<Longrightarrow> bij \<sigma>' \<Longrightarrow>
-  (\<forall>x \<in> PTVars P. \<tau> x = \<tau>' x) \<Longrightarrow> (\<forall>x \<in> PVars P. \<sigma> x = \<sigma>' x) \<Longrightarrow>  
-  tvsubst_pat \<tau> \<sigma> P = tvsubst_pat \<tau>' \<sigma>' P"
-  by transfer (auto simp: tvsubst_prepat_cong)
+  shows "|SSupp_type \<tau>| <o |UNIV :: 'tv::var set| \<Longrightarrow> |SSupp_type \<tau>'| <o |UNIV :: 'tv::var set| \<Longrightarrow> bij \<sigma> \<Longrightarrow> bij \<sigma>' \<Longrightarrow>
+  (\<forall>x \<in> PTV P. \<tau> x = \<tau>' x) \<Longrightarrow> (\<forall>x \<in> PV P. \<sigma> x = \<sigma>' x) \<Longrightarrow>  
+  subst_pat \<tau> \<sigma> P = subst_pat \<tau>' \<sigma>' P"
+  by transfer (auto simp: subst_ppat_cong)
 
 lemma vvsubst_pat_id[simp]: "vvsubst_pat id id P = P"
   apply transfer
   subgoal for P
     apply (induct P)
-     apply (force simp: typ.map_id values_lfin_iff intro!: trans[OF lfset.map_cong_id lfset.map_id])+
+     apply (force simp: type.map_id values_lfin_iff intro!: trans[OF lfset.map_cong_id lfset.map_id])+
     done
   done
 
 mrbnf "('tv :: var, 'v :: var) pat"
   map: vvsubst_pat
   sets:
-    free: PTVars
-    bound: "PVars"
+    free: PTV
+    bound: "PV"
   bd: "natLeq"
   rel: "(=)"
   subgoal
@@ -341,14 +341,14 @@ mrbnf "('tv :: var, 'v :: var) pat"
     apply (transfer fixing: f1 f2 g1 g2)
     subgoal for P
       apply (induct P)
-       apply (force simp: typ.map_comp lfset.map_comp values_lfin_iff intro!: lfset.map_cong)+
+       apply (force simp: type.map_comp lfset.map_comp values_lfin_iff intro!: lfset.map_cong)+
       done
     done
   subgoal for P f1 f2 g1 g2
     apply (transfer fixing: f1 f2 g1 g2)
     subgoal for P
       apply (induct P)
-       apply (fastforce simp: values_lfin_iff Bex_def intro!: typ.map_cong lfset.map_cong)+
+       apply (fastforce simp: values_lfin_iff Bex_def intro!: type.map_cong lfset.map_cong)+
       done
     done
   subgoal for f g
@@ -356,7 +356,7 @@ mrbnf "('tv :: var, 'v :: var) pat"
     apply (transfer fixing: f g)
     subgoal for P
       apply (induct P)
-       apply (fastforce simp: typ.set_map lfset.set_map values_lfin_iff)+
+       apply (fastforce simp: type.set_map lfset.set_map values_lfin_iff)+
       done
     done
   subgoal for f g
@@ -364,7 +364,7 @@ mrbnf "('tv :: var, 'v :: var) pat"
     apply (transfer fixing: f g)
     subgoal for P
       apply (induct P)
-       apply (fastforce simp: typ.set_map lfset.set_map values_lfin_iff)+
+       apply (fastforce simp: type.set_map lfset.set_map values_lfin_iff)+
       done
     done
   subgoal by (simp add: infinite_regular_card_order_natLeq)
@@ -372,14 +372,14 @@ mrbnf "('tv :: var, 'v :: var) pat"
     apply transfer
     subgoal for P
     apply (induct P)
-       apply (force simp: typ.FVars_bd lfset.set_bd values_lfin_iff intro!: stable_UNION[OF stable_natLeq])+
+       apply (force simp: type.FVars_bd lfset.set_bd values_lfin_iff intro!: stable_UNION[OF stable_natLeq])+
       done
     done
   subgoal for P
     apply transfer
     subgoal for P
     apply (induct P)
-       apply (force simp: typ.FVars_bd lfset.set_bd ID.set_bd values_lfin_iff intro!: stable_UNION[OF stable_natLeq])+
+       apply (force simp: type.FVars_bd lfset.set_bd ID.set_bd values_lfin_iff intro!: stable_UNION[OF stable_natLeq])+
       done
     done
   subgoal by simp
@@ -387,17 +387,17 @@ mrbnf "('tv :: var, 'v :: var) pat"
   done
 
 lemma vvsubst_pat_PVar[simp]:
-  "bij g \<Longrightarrow> vvsubst_pat f g (PVar x T) = PVar (g x) (vvsubst_typ f T)"
+  "bij g \<Longrightarrow> vvsubst_pat f g (PVr x T) = PVr (g x) (vvsubst_type f T)"
   by transfer auto
-lemma tvsubst_pat_PVar[simp]:
-  "bij g \<Longrightarrow> tvsubst_pat f g (PVar x T) = PVar (g x) (tvsubst_typ f T)"
+lemma subst_pat_PVar[simp]:
+  "bij g \<Longrightarrow> subst_pat f g (PVr x T) = PVr (g x) (substT f T)"
   by transfer auto
 
-definition "nonrep_PRec X = (\<forall>x y P Q. x \<noteq> y \<longrightarrow> (x, P) \<in>\<in> X \<longrightarrow> (y, Q) \<in>\<in> X \<longrightarrow> PVars P \<inter> PVars Q = {})"
+definition "nonrep_PRec X = (\<forall>x y P Q. x \<noteq> y \<longrightarrow> (x, P) \<in>\<in> X \<longrightarrow> (y, Q) \<in>\<in> X \<longrightarrow> PV P \<inter> PV Q = {})"
 
 lemma nonrep_PRec_alt: "nonrep_PRec X = nonrep_PPRec (map_lfset id Rep_pat X)"
   unfolding nonrep_PRec_def nonrep_PPRec_def
-  apply (auto simp: PVars_def)
+  apply (auto simp: PV_def)
    apply (metis Int_emptyD lfin_map_lfset)
   apply (meson Int_emptyD lfin_map_lfset)
   done
@@ -416,57 +416,57 @@ lemma vvsubst_pat_PRec[simp]:
   unfolding PRec_def vvsubst_pat_def nonrep_PRec_alt
   apply (auto simp: lfset.map_comp o_def map_fun_def id_def[symmetric])
      apply (subst (1 2) Abs_pat_inverse)
-  using Rep_pat nonrep_prepat_vvsubst_prepat apply blast
+  using Rep_pat nonrep_ppat_vvsubst_ppat apply blast
   apply (auto) []
       apply (metis Rep_pat lfin_map_lfset mem_Collect_eq)
      apply (subst Abs_pat_inject)
-  apply (metis (mono_tags, lifting) Rep_pat lfin_map_lfset mem_Collect_eq nonrep_prepat_PRec
-      nonrep_prepat_vvsubst_prepat)
+  apply (metis (mono_tags, lifting) Rep_pat lfin_map_lfset mem_Collect_eq nonrep_ppat_PRec
+      nonrep_ppat_vvsubst_ppat)
   apply (smt (verit, best) Abs_pat_inverse Rep_pat lfin_map_lfset lfset.map_cong_id
-      mem_Collect_eq nonrep_prepat_PRec nonrep_prepat_vvsubst_prepat)
+      mem_Collect_eq nonrep_ppat_PRec nonrep_ppat_vvsubst_ppat)
      apply (auto simp: lfset.map_comp intro!: lfset.map_cong) []
   apply (smt (z3) Abs_pat_inverse Rep_pat lfin_map_lfset mem_Collect_eq nonrep_PPRec_def
-      nonrep_prepat_PRec nonrep_prepat_vvsubst_prepat
-      vvsubst_prepat.simps(2))
+      nonrep_ppat_PRec nonrep_ppat_vvsubst_ppat
+      vvsubst_ppat.simps(2))
   done
 
-lemma tvsubst_pat_PRec[simp]:
-  "bij g \<Longrightarrow> nonrep_PRec P \<Longrightarrow> tvsubst_pat f g (PRec P) = PRec (map_lfset id (tvsubst_pat f g) P)"
-  unfolding PRec_def tvsubst_pat_def nonrep_PRec_alt
+lemma subst_pat_PRec[simp]:
+  "bij g \<Longrightarrow> nonrep_PRec P \<Longrightarrow> subst_pat f g (PRec P) = PRec (map_lfset id (subst_pat f g) P)"
+  unfolding PRec_def subst_pat_def nonrep_PRec_alt
   apply (auto simp: lfset.map_comp o_def map_fun_def id_def[symmetric])
      apply (subst (1 2) Abs_pat_inverse)
-  using Rep_pat nonrep_prepat_tvsubst_prepat apply blast
+  using Rep_pat nonrep_ppat_subst_ppat apply blast
   apply (auto) []
       apply (metis Rep_pat lfin_map_lfset mem_Collect_eq)
      apply (subst Abs_pat_inject)
-  apply (metis (mono_tags, lifting) Rep_pat lfin_map_lfset mem_Collect_eq nonrep_prepat_PRec
-      nonrep_prepat_tvsubst_prepat)
+  apply (metis (mono_tags, lifting) Rep_pat lfin_map_lfset mem_Collect_eq nonrep_ppat_PRec
+      nonrep_ppat_subst_ppat)
   apply (smt (verit, best) Abs_pat_inverse Rep_pat lfin_map_lfset lfset.map_cong_id
-      mem_Collect_eq nonrep_prepat_PRec nonrep_prepat_tvsubst_prepat)
+      mem_Collect_eq nonrep_ppat_PRec nonrep_ppat_subst_ppat)
      apply (auto simp: lfset.map_comp intro!: lfset.map_cong) []
   apply (smt (z3) Abs_pat_inverse Rep_pat lfin_map_lfset mem_Collect_eq nonrep_PPRec_def
-      nonrep_prepat_PRec nonrep_prepat_tvsubst_prepat
-      tvsubst_prepat.simps(2))
+      nonrep_ppat_PRec nonrep_ppat_subst_ppat
+      subst_ppat.simps(2))
   done
 
-lemma PVars_PVar[simp]: "PVars (PVar x T) = {x}"
-  by (auto simp: PVars_def PVar_def Abs_pat_inverse)
-lemma PVars_PRec[simp]: "nonrep_PRec P \<Longrightarrow> PVars (PRec P) = (\<Union>x \<in> values P. PVars x)"
-  apply (auto simp: PVars_def PRec_def Abs_pat_inverse nonrep_PRec_alt lfin_map_lfset lfset.set_map Rep_pat[simplified])
+lemma PV_PVar[simp]: "PV (PVr x T) = {x}"
+  by (auto simp: PV_def PVr_def Abs_pat_inverse)
+lemma PV_PRec[simp]: "nonrep_PRec P \<Longrightarrow> PV (PRec P) = (\<Union>x \<in> values P. PV x)"
+  apply (auto simp: PV_def PRec_def Abs_pat_inverse nonrep_PRec_alt lfin_map_lfset lfset.set_map Rep_pat[simplified])
    apply (subst (asm) Abs_pat_inverse; auto simp: lfin_map_lfset Rep_pat[simplified] lfset.set_map)
    apply (subst Abs_pat_inverse; auto simp: lfin_map_lfset Rep_pat[simplified] lfset.set_map)
   done
-lemma PTVars_PVar[simp]: "PTVars (PVar x T) = FVars_typ T"
-  by (auto simp: PTVars_def PVar_def Abs_pat_inverse)
-lemma PTVars_PRec[simp]: "nonrep_PRec P \<Longrightarrow> PTVars (PRec P) = (\<Union>x \<in> values P. PTVars x)"
-  apply (auto simp: PTVars_def PRec_def Abs_pat_inverse nonrep_PRec_alt lfin_map_lfset lfset.set_map Rep_pat[simplified])
+lemma PTV_PVar[simp]: "PTV (PVr x T) = TFV T"
+  by (auto simp: PTV_def PVr_def Abs_pat_inverse)
+lemma PTV_PRec[simp]: "nonrep_PRec P \<Longrightarrow> PTV (PRec P) = (\<Union>x \<in> values P. PTV x)"
+  apply (auto simp: PTV_def PRec_def Abs_pat_inverse nonrep_PRec_alt lfin_map_lfset lfset.set_map Rep_pat[simplified])
    apply (subst (asm) Abs_pat_inverse; auto simp: lfin_map_lfset Rep_pat[simplified] lfset.set_map)
    apply (subst Abs_pat_inverse; auto simp: lfin_map_lfset Rep_pat[simplified] lfset.set_map)
   done
 
-lemma finite_PVars[simp]: "finite (PVars P)"
-  by (auto simp: PVars_def finite_PPVars)
-lemma finite_PTVars[simp]: "finite (PTVars P)"
-  by (auto simp: PTVars_def finite_PPTVars)
+lemma finite_PV[simp]: "finite (PV P)"
+  by (auto simp: PV_def finite_PPV)
+lemma finite_PTV[simp]: "finite (PTV P)"
+  by (auto simp: PTV_def finite_PPTV)
 
 end
