thys/POPLmark/SystemFSub.thy
@@ -3,7 +3,6 @@ theory SystemFSub
   imports "Binders.MRBNF_Recursor"
     "Binders.Generic_Barendregt_Enhanced_Rule_Induction"
     "Prelim.Curry_LFP"
-    "Prelim.FixedCountableVars"
     "Labeled_FSet"
 begin
 
@@ -12,24 +11,25 @@ declare supp_id_bound[simp]
 type_synonym label = string
 
 declare [[mrbnf_internals]]
-binder_datatype 'a "typ" =
-    TyVar 'a
+binder_datatype (TFV: 'tvar) "type" =
+    TVr 'tvar
   | Top
-  | Fun "'a typ" "'a typ"
-  | Forall \<alpha>::'a "'a typ" t::"'a typ" binds \<alpha> in t
-  | TRec "(label, 'a typ) lfset"
+  | Arr "'tvar type" "'tvar type"
+  | All X::'tvar "'tvar type" T::"'tvar type" binds X in T
+  | TRec "(label, 'tvar type) lfset"
+  for tvsubst : substT
 
-declare supp_swap_bound[OF cinfinite_imp_infinite[OF typ.UNIV_cinfinite], simp]
-declare typ.permute_id[simp] typ.permute_id0[simp]
+declare supp_swap_bound[OF cinfinite_imp_infinite[OF type.UNIV_cinfinite], simp]
+declare type.permute_id[simp] type.permute_id0[simp]
 
-lemma Forall_rrename:
+lemma All_rrename:
   assumes "bij \<sigma>" "|supp \<sigma>| <o |UNIV::'a set|" shows "
- (\<And>a'. a'\<in>FVars_typ T2 - {x::'a::var} \<Longrightarrow> \<sigma> a' = a') \<Longrightarrow> Forall x T1 T2 = Forall (\<sigma> x) T1 (permute_typ \<sigma> T2)"
-  apply (unfold Forall_def)
-  apply (unfold typ.TT_inject0)
-  apply (unfold set3_typ_pre_def set2_typ_pre_def comp_def Abs_typ_pre_inverse[OF UNIV_I] map_sum.simps
+ (\<And>a'. a'\<in>TFV T2 - {x::'a::var} \<Longrightarrow> \<sigma> a' = a') \<Longrightarrow> All x T1 T2 = All (\<sigma> x) T1 (permute_type \<sigma> T2)"
+  apply (unfold All_def)
+  apply (unfold type.TT_inject0)
+  apply (unfold set3_type_pre_def set2_type_pre_def comp_def Abs_type_pre_inverse[OF UNIV_I] map_sum.simps
     map_prod_simp sum_set_simps prod_set_simps cSup_singleton Un_empty_left Un_empty_right
-    Union_empty image_insert image_empty map_typ_pre_def id_def)
+    Union_empty image_insert image_empty map_type_pre_def id_def)
   apply (rule exI[of _ \<sigma>])
   apply (rule conjI assms)+
    apply (unfold id_on_def atomize_all atomize_imp)[1]
@@ -38,18 +38,18 @@ lemma Forall_rrename:
   apply (rule refl)
   done
 
-lemma Forall_swapD: "Forall (x::'a::var) T1 T2 = Forall y T1' T2' \<Longrightarrow> T1 = T1' \<and> T2' = permute_typ (x \<leftrightarrow> y) T2"
-  unfolding typ.inject
-  by (auto intro!: typ.permute_cong simp: id_on_def)
+lemma All_swapD: "All (x::'a::var) T1 T2 = All y T1' T2' \<Longrightarrow> T1 = T1' \<and> T2' = permute_type (x \<leftrightarrow> y) T2"
+  unfolding type.inject
+  by (auto intro!: type.permute_cong simp: id_on_def)
 
-type_synonym ('a, 'b) \<Gamma> = "('b \<times> 'a typ) list"
+type_synonym ('a, 'b) \<Gamma> = "('b \<times> 'a type) list"
 type_synonym 'a \<Gamma>\<^sub>\<tau> = "('a, 'a) \<Gamma>"
 
 definition map_context :: "('a::var \<Rightarrow> 'a) \<Rightarrow> 'a \<Gamma>\<^sub>\<tau> \<Rightarrow> 'a \<Gamma>\<^sub>\<tau>" where
-  "map_context f \<equiv> map (map_prod f (permute_typ f))"
+  "map_context f \<equiv> map (map_prod f (permute_type f))"
 abbreviation FFVars_ctxt :: "('a::var, 'b) \<Gamma> \<Rightarrow> 'a set" where
-  "FFVars_ctxt xs \<equiv> \<Union>(FVars_typ ` snd ` set xs)"
-abbreviation extend :: "('a, 'b) \<Gamma> \<Rightarrow> 'b \<Rightarrow> 'a typ \<Rightarrow> ('a, 'b) \<Gamma>" ("_ \<^bold>, _ <: _" [57,75,75] 71) where
+  "FFVars_ctxt xs \<equiv> \<Union>(TFV ` snd ` set xs)"
+abbreviation extend :: "('a, 'b) \<Gamma> \<Rightarrow> 'b \<Rightarrow> 'a type \<Rightarrow> ('a, 'b) \<Gamma>" ("_ \<^bold>, _ <: _" [57,75,75] 71) where
   "extend \<Gamma> x T \<equiv> (x, T)#\<Gamma>"
 abbreviation concat :: "('a, 'b) \<Gamma> \<Rightarrow> ('a, 'b) \<Gamma> \<Rightarrow> ('a, 'b) \<Gamma>" (infixl "(\<^bold>,)" 71) where
   "concat \<Gamma> \<Delta> \<equiv> \<Delta> @ \<Gamma>"
@@ -65,7 +65,7 @@ lemma map_context_comp0[simp]:
   shows "map_context f \<circ> map_context g = map_context (f \<circ> g)"
   apply (rule ext)
   unfolding map_context_def
-  using assms by (auto simp: typ.permute_comp)
+  using assms by (auto simp: type.permute_comp)
 lemmas map_context_comp = trans[OF comp_apply[symmetric] fun_cong[OF map_context_comp0]]
 declare map_context_comp[simp]
 lemma context_dom_set[simp]:
@@ -76,7 +76,7 @@ lemma context_dom_set[simp]:
 lemma set_bd_UNIV: "|set xs| <o |UNIV::'a::var set|"
   apply (rule ordLess_ordLeq_trans)
    apply (rule list.set_bd)
-  apply (rule typ_pre.var_large)
+  apply (rule type_pre.var_large)
   done
 lemma context_set_bd_UNIV[simp]: "|dom xs| <o |UNIV::'a::var set|"
   apply (rule ordLeq_ordLess_trans[OF card_of_image])
@@ -90,15 +90,15 @@ shows "map_context f \<Gamma> = \<Gamma>"
    apply (rule list.map_cong0[of _ _ id])
    apply (rule trans)
     apply (rule prod.map_cong0[of _ _ id _ id])
-  using assms by (fastforce intro!: typ.permute_cong_id)+
+  using assms by (fastforce intro!: type.permute_cong_id)+
 
-notation Fun (infixr "\<rightarrow>" 65)
-notation Forall ("\<forall> _ <: _ . _" [62, 62, 62] 70)
+notation Arr (infixr "\<rightarrow>" 65)
+notation All ("\<forall> _ <: _ . _" [62, 62, 62] 70)
 
-abbreviation in_context :: "'a \<Rightarrow> 'a typ \<Rightarrow> 'a \<Gamma>\<^sub>\<tau> \<Rightarrow> bool" ("_ <: _ \<in> _" [55,55,55] 60) where
+abbreviation in_context :: "'a \<Rightarrow> 'a type \<Rightarrow> 'a \<Gamma>\<^sub>\<tau> \<Rightarrow> bool" ("_ <: _ \<in> _" [55,55,55] 60) where
   "x <: t \<in> \<Gamma> \<equiv> (x, t) \<in> set \<Gamma>"
-abbreviation well_scoped :: "'a::var typ \<Rightarrow> 'a \<Gamma>\<^sub>\<tau> \<Rightarrow> bool" ("_ closed'_in _" [55, 55] 60) where
-  "well_scoped S \<Gamma> \<equiv> FVars_typ S \<subseteq> dom \<Gamma>"
+abbreviation well_scoped :: "'a::var type \<Rightarrow> 'a \<Gamma>\<^sub>\<tau> \<Rightarrow> bool" ("_ closed'_in _" [55, 55] 60) where
+  "well_scoped S \<Gamma> \<equiv> TFV S \<subseteq> dom \<Gamma>"
 
 inductive wf_ty :: "'a::var \<Gamma>\<^sub>\<tau> \<Rightarrow> bool" ("\<turnstile> _ ok" [70] 100) where
   wf_Nil[intro]: "\<turnstile> [] ok"
@@ -111,25 +111,25 @@ inductive_cases
 lemma in_context_eqvt:
   fixes f::"'a::var \<Rightarrow> 'a"
   assumes "bij f" "|supp f| <o |UNIV::'a set|"
-  shows "x <: T \<in> \<Gamma> \<Longrightarrow> f x <: permute_typ f T \<in> map_context f \<Gamma>"
+  shows "x <: T \<in> \<Gamma> \<Longrightarrow> f x <: permute_type f T \<in> map_context f \<Gamma>"
   using assms unfolding map_context_def by auto
 
 lemma extend_eqvt:
   fixes f::"'a::var \<Rightarrow> 'a"
   assumes "bij f" "|supp f| <o |UNIV::'a set|"
-  shows "map_context f (\<Gamma>\<^bold>,x<:T) = map_context f \<Gamma>\<^bold>, f x <: permute_typ f T"
+  shows "map_context f (\<Gamma>\<^bold>,x<:T) = map_context f \<Gamma>\<^bold>, f x <: permute_type f T"
   unfolding map_context_def by simp
 
 lemma extend_equiv[equiv]:
   fixes f1::"'a::var \<Rightarrow> 'a" and f2::"'b::var \<Rightarrow> 'b"
   assumes "bij f1" "bij f2"
-  shows "map (map_prod f1 (permute_typ f2)) (\<Gamma>\<^bold>,x<:T) = map (map_prod f1 (permute_typ f2)) \<Gamma>\<^bold>, f1 x <: permute_typ f2 T"
+  shows "map (map_prod f1 (permute_type f2)) (\<Gamma>\<^bold>,x<:T) = map (map_prod f1 (permute_type f2)) \<Gamma>\<^bold>, f1 x <: permute_type f2 T"
   by simp
 
 lemma closed_in_eqvt:
   assumes "bij (f::'a \<Rightarrow> 'a)" "|supp f| <o |UNIV::'a::var set|"
-  shows "S closed_in \<Gamma> \<Longrightarrow> permute_typ f S closed_in map_context f \<Gamma>"
-  using assms  by (auto simp: typ.FVars_permute)
+  shows "S closed_in \<Gamma> \<Longrightarrow> permute_type f S closed_in map_context f \<Gamma>"
+  using assms  by (auto simp: type.FVars_permute)
 
 lemma wf_eqvt:
   fixes f::"'a::var \<Rightarrow> 'a"
@@ -142,11 +142,11 @@ unfolding map_context_def proof (induction \<Gamma>)
     by (metis (no_types, lifting) closed_in_eqvt list.set_map map_context_def subsetD)
 qed simp
 
-abbreviation Tsupp :: "'a::var \<Gamma>\<^sub>\<tau> \<Rightarrow> 'a typ \<Rightarrow> 'a typ \<Rightarrow> 'a set" where
-  "Tsupp \<Gamma> T\<^sub>1 T\<^sub>2 \<equiv> dom \<Gamma> \<union> FFVars_ctxt \<Gamma> \<union> FVars_typ T\<^sub>1 \<union> FVars_typ T\<^sub>2"
+abbreviation Tsupp :: "'a::var \<Gamma>\<^sub>\<tau> \<Rightarrow> 'a type \<Rightarrow> 'a type \<Rightarrow> 'a set" where
+  "Tsupp \<Gamma> T\<^sub>1 T\<^sub>2 \<equiv> dom \<Gamma> \<union> FFVars_ctxt \<Gamma> \<union> TFV T\<^sub>1 \<union> TFV T\<^sub>2"
 
 lemma small_Tsupp: "small (Tsupp x1 x2 x3)"
-  by (auto simp: small_def typ.set_bd_UNIV typ.Un_bound var_class.UN_bound set_bd_UNIV typ.set_bd)
+  by (auto simp: small_def type.set_bd_UNIV type.Un_bound var_class.UN_bound set_bd_UNIV type.set_bd)
 
 lemma fresh: "\<exists>xx. xx \<notin> Tsupp x1 x2 x3"
   using exists_fresh small_Tsupp small_def by blast
@@ -158,7 +158,7 @@ lemma wf_FFVars: "\<turnstile> \<Gamma> ok \<Longrightarrow> a \<in> FFVars_ctxt
   by (induction \<Gamma>) auto
 
 lemma finite_Tsupp: "finite (Tsupp x1 x2 x3)"
-  using finite_iff_ordLess_natLeq typ.set_bd by fastforce
+  using finite_iff_ordLess_natLeq type.set_bd by fastforce
 
 lemma exists_fresh:
 "\<exists> z. z \<notin> set xs \<and> z \<notin> Tsupp x1 x2 x3"
@@ -170,23 +170,23 @@ proof-
   thus ?thesis by auto
 qed
 
-lemma rrename_swap_FFvars[simp]: "x \<notin> FVars_typ T \<Longrightarrow> xx \<notin> FVars_typ T \<Longrightarrow>
-  permute_typ (x \<leftrightarrow> xx) T = T"
-apply(rule typ.permute_cong_id) apply auto by (metis swap_def)
+lemma rrename_swap_FFvars[simp]: "x \<notin> TFV T \<Longrightarrow> xx \<notin> TFV T \<Longrightarrow>
+  permute_type (x \<leftrightarrow> xx) T = T"
+apply(rule type.permute_cong_id) apply auto by (metis swap_def)
 
 lemma map_context_swap_FFVars[simp]:
-"\<forall>k\<in>set \<Gamma>. x \<noteq> fst k \<and> x \<notin> FVars_typ (snd k) \<and>
-           xx \<noteq> fst k \<and> xx \<notin> FVars_typ (snd k) \<Longrightarrow>
+"\<forall>k\<in>set \<Gamma>. x \<noteq> fst k \<and> x \<notin> TFV (snd k) \<and>
+           xx \<noteq> fst k \<and> xx \<notin> TFV (snd k) \<Longrightarrow>
     map_context (x \<leftrightarrow> xx) \<Gamma> = \<Gamma>"
   unfolding map_context_def apply(rule map_idI) by auto
 
 lemma isPerm_swap: "isPerm (x \<leftrightarrow> xx)"
   unfolding isPerm_def by (auto simp: infinite_UNIV)
 
-inductive ty :: "'a::var \<Gamma>\<^sub>\<tau> \<Rightarrow> 'a typ \<Rightarrow> 'a typ \<Rightarrow> bool" ("_ \<turnstile> _ <: _" [55,55,55] 60) where
+inductive ty :: "'a::var \<Gamma>\<^sub>\<tau> \<Rightarrow> 'a type \<Rightarrow> 'a type \<Rightarrow> bool" ("_ \<turnstile> _ <: _" [55,55,55] 60) where
   SA_Top: "\<lbrakk> \<turnstile> \<Gamma> ok ; S closed_in \<Gamma> \<rbrakk> \<Longrightarrow> \<Gamma> \<turnstile> S <: Top"
-| SA_Refl_TVar: "\<lbrakk> \<turnstile> \<Gamma> ok ; TyVar x closed_in \<Gamma> \<rbrakk> \<Longrightarrow> \<Gamma> \<turnstile> TyVar x <: TyVar x"
-| SA_Trans_TVar: "\<lbrakk> x<:U \<in> \<Gamma> ; \<Gamma> \<turnstile> U <: T \<rbrakk> \<Longrightarrow> \<Gamma> \<turnstile> TyVar x <: T"
+| SA_Refl_TVar: "\<lbrakk> \<turnstile> \<Gamma> ok ; TVr x closed_in \<Gamma> \<rbrakk> \<Longrightarrow> \<Gamma> \<turnstile> TVr x <: TVr x"
+| SA_Trans_TVar: "\<lbrakk> x<:U \<in> \<Gamma> ; \<Gamma> \<turnstile> U <: T \<rbrakk> \<Longrightarrow> \<Gamma> \<turnstile> TVr x <: T"
 | SA_Arrow: "\<lbrakk> \<Gamma> \<turnstile> T\<^sub>1 <: S\<^sub>1 ; \<Gamma> \<turnstile> S\<^sub>2 <: T\<^sub>2 \<rbrakk> \<Longrightarrow> \<Gamma> \<turnstile> S\<^sub>1 \<rightarrow> S\<^sub>2 <: T\<^sub>1 \<rightarrow> T\<^sub>2"
 | SA_All: "\<lbrakk> \<Gamma> \<turnstile> T\<^sub>1 <: S\<^sub>1 ; \<Gamma>\<^bold>, x<:T\<^sub>1 \<turnstile> S\<^sub>2 <: T\<^sub>2 \<rbrakk> \<Longrightarrow> \<Gamma> \<turnstile> \<forall>x<:S\<^sub>1. S\<^sub>2 <: \<forall>x<:T\<^sub>1 .T\<^sub>2"
 | SA_TRec: "\<lbrakk> \<turnstile> \<Gamma> ok; labels Y \<subseteq> labels X;
@@ -196,7 +196,7 @@ inductive ty :: "'a::var \<Gamma>\<^sub>\<tau> \<Rightarrow> 'a typ \<Rightarrow
 inductive_cases
   SA_TopE[elim!]: "\<Gamma> \<turnstile> Top <: T"
 and
-  SA_TVarE: "\<Gamma> \<turnstile> S <: TyVar Z"
+  SA_TVarE: "\<Gamma> \<turnstile> S <: TVr Z"
 and
   SA_ArrER: "\<Gamma> \<turnstile> S <: T\<^sub>1 \<rightarrow> T\<^sub>2"
 and
@@ -220,7 +220,7 @@ using assms proof (induction \<Gamma> S T rule: ty.induct)
   case (SA_Trans_TVar x U \<Gamma> T)
   {
     case 1 then show ?case using SA_Trans_TVar
-      by (metis fst_conv imageI singletonD subsetI typ.set(1))
+      by (metis fst_conv imageI singletonD subsetI type.set(1))
   next
     case 2 then show ?case using SA_Trans_TVar by simp
   }
@@ -228,24 +228,24 @@ next
   case (SA_TRec \<Gamma> Y X)
   {
     case 1
-    then show ?case unfolding typ.set
+    then show ?case unfolding type.set
     proof safe
       fix x T
-      assume a: "T \<in> values X" "x \<in> FVars_typ T"
+      assume a: "T \<in> values X" "x \<in> TFV T"
       from \<open>T \<in> values X\<close> obtain l where 1: "(l, T) \<in>\<in> X"
         by (meson values_lfin)
       then show "x \<in> dom \<Gamma>" using SA_TRec(3) a by fast
     qed
   next
     case 2
-    then show ?case unfolding typ.set
+    then show ?case unfolding type.set
       by (auto dest!: values_lfin SA_TRec(4))
   }
 qed auto
 
 declare ty.intros[intro]
 
-lemma ty_fresh_extend: "\<Gamma>\<^bold>, x <: U \<turnstile> S <: T \<Longrightarrow> x \<notin> dom \<Gamma> \<union> FFVars_ctxt \<Gamma> \<and> x \<notin> FVars_typ U"
+lemma ty_fresh_extend: "\<Gamma>\<^bold>, x <: U \<turnstile> S <: T \<Longrightarrow> x \<notin> dom \<Gamma> \<union> FFVars_ctxt \<Gamma> \<and> x \<notin> TFV U"
   by (metis (no_types, lifting) UnE fst_conv snd_conv subsetD wf_ConsE wf_FFVars wf_context)
 
 declare wf_eqvt[unfolded map_context_def, equiv]
@@ -258,154 +258,154 @@ thm equiv
 thm equiv_sym
 thm equiv_forward
 
-lemma typ_inject: "Forall x T1 T2 = Forall y R1 R2 \<longleftrightarrow> T1 = R1 \<and> (\<exists>f. bij (f::'a::var \<Rightarrow> 'a) \<and> |supp f| <o |UNIV::'a set| \<and> id_on (FVars_typ T2 - {x}) f \<and> f x = y \<and> permute_typ f T2 = R2)"
-  by (smt (z3) Forall_rrename Swapping.bij_swap Swapping.supp_swap_bound id_on_def id_on_swap infinite_UNIV swap_simps(1) typ.inject(3))
+lemma type_inject: "All x T1 T2 = All y R1 R2 \<longleftrightarrow> T1 = R1 \<and> (\<exists>f. bij (f::'a::var \<Rightarrow> 'a) \<and> |supp f| <o |UNIV::'a set| \<and> id_on (TFV T2 - {x}) f \<and> f x = y \<and> permute_type f T2 = R2)"
+  by (smt (z3) All_rrename Swapping.bij_swap Swapping.supp_swap_bound id_on_def id_on_swap infinite_UNIV swap_simps(1) type.inject(3))
 
-lemmas typ.inject(3)[simp del]
+lemmas type.inject(3)[simp del]
 binder_inductive ty
   subgoal premises prems for R B \<Gamma> T1 T2
     by (tactic \<open>refreshability_tac false
-      [@{term "\<lambda>(\<Gamma>::('a::var \<times> 'a typ) list). dom \<Gamma> \<union> FFVars_ctxt \<Gamma>"}, @{term "FVars_typ :: 'a typ \<Rightarrow> 'a::var set"}, @{term "FVars_typ :: 'a::var typ \<Rightarrow> 'a::var set"}]
-      [@{term "permute_typ :: ('a::var \<Rightarrow> 'a) \<Rightarrow> 'a typ \<Rightarrow> 'a typ"}, @{term "(\<lambda>f x. f x) :: ('a::var \<Rightarrow> 'a) \<Rightarrow> 'a \<Rightarrow> 'a"}]
+      [@{term "\<lambda>(\<Gamma>::('a::var \<times> 'a type) list). dom \<Gamma> \<union> FFVars_ctxt \<Gamma>"}, @{term "TFV :: 'a type \<Rightarrow> 'a::var set"}, @{term "TFV :: 'a::var type \<Rightarrow> 'a::var set"}]
+      [@{term "permute_type :: ('a::var \<Rightarrow> 'a) \<Rightarrow> 'a type \<Rightarrow> 'a type"}, @{term "(\<lambda>f x. f x) :: ('a::var \<Rightarrow> 'a) \<Rightarrow> 'a \<Rightarrow> 'a"}]
       [NONE, NONE, NONE, NONE, SOME [NONE, NONE, NONE, SOME 1, SOME 0, SOME 0], NONE]
       @{thm prems(3)} @{thm prems(2)} @{thms prems(1)[THEN ty_fresh_extend] id_onD}
-      @{thms emp_bound insert_bound ID.set_bd typ.Un_bound typ.UN_bound typ.set_bd_UNIV infinite_UNIV}
-      @{thms typ_inject image_iff} @{thms typ.permute_cong_id context_map_cong_id map_idI}
+      @{thms emp_bound insert_bound ID.set_bd type.Un_bound type.UN_bound type.set_bd_UNIV infinite_UNIV}
+      @{thms type_inject image_iff} @{thms type.permute_cong_id context_map_cong_id map_idI}
       @{thms cong[OF cong[OF cong[OF refl[of R]] refl] refl, THEN iffD1, rotated -1] id_onD} @{context}\<close>)
   done
 
-lemma VVr_eq_TyVar[simp]: "tvVVr_tvsubst_typ a = TyVar a"
-  unfolding tvVVr_tvsubst_typ_def comp_def tv\<eta>_typ_tvsubst_typ_def TyVar_def
+lemma VVr_eq_TVr[simp]: "tvVVr_substT a = TVr a"
+  unfolding tvVVr_substT_def comp_def tv\<eta>_type_substT_def TVr_def
   by (rule refl)
 
-lemma FVars_tvsubst_typ:
-  assumes "|SSupp_typ (g::'tv \<Rightarrow> _)| <o |UNIV::'tv::var set|"
-  shows "FVars_typ (tvsubst_typ g x) = \<Union>((FVars_typ \<circ> g) ` FVars_typ x)"
-proof (binder_induction x avoiding: x "IImsupp_typ g" rule: typ.strong_induct)
+lemma FVars_substT:
+  assumes "|SSupp_type (g::'tv \<Rightarrow> _)| <o |UNIV::'tv::var set|"
+  shows "TFV (substT g x) = \<Union>((TFV \<circ> g) ` TFV x)"
+proof (binder_induction x avoiding: x "IImsupp_type g" rule: type.strong_induct)
   case Bound
-  then show ?case unfolding IImsupp_typ_def using var_class.Un_bound var_class.UN_bound typ.set_bd_UNIV assms
+  then show ?case unfolding IImsupp_type_def using var_class.Un_bound var_class.UN_bound type.set_bd_UNIV assms
     by (metis type_copy_set_bd)
 next
-  case (Forall x1 x2 x3)
+  case (All x1 x2 x3)
   then show ?case apply (auto simp: assms)
-    using IImsupp_typ_def SSupp_typ_def typ.FVars_VVr apply fastforce
-    by (metis singletonD typ.FVars_VVr typ.in_IImsupp)
+    using IImsupp_type_def SSupp_type_def type.FVars_VVr apply fastforce
+    by (metis singletonD type.FVars_VVr type.in_IImsupp)
 qed (auto simp: lfset.set_map assms)
 
-lemma SSupp_typ_TyVar_comp: "SSupp_typ (TyVar o \<sigma>) = supp \<sigma>"
-  unfolding SSupp_typ_def supp_def by auto
+lemma SSupp_type_TVr_comp: "SSupp_type (TVr o \<sigma>) = supp \<sigma>"
+  unfolding SSupp_type_def supp_def by auto
 
-lemma IImsupp_typ_TyVar_comp: "IImsupp_typ (TyVar o \<sigma>) = imsupp \<sigma>"
-  unfolding IImsupp_typ_def imsupp_def SSupp_typ_TyVar_comp by auto
+lemma IImsupp_type_TVr_comp: "IImsupp_type (TVr o \<sigma>) = imsupp \<sigma>"
+  unfolding IImsupp_type_def imsupp_def SSupp_type_TVr_comp by auto
 
-lemma SSupp_typ_TyVar[simp]: "SSupp_typ TyVar = {}"
-  unfolding SSupp_typ_def by simp
+lemma SSupp_type_TVr[simp]: "SSupp_type TVr = {}"
+  unfolding SSupp_type_def by simp
 
-lemma IImsupp_typ_TyVar[simp]: "IImsupp_typ TyVar = {}"
-  unfolding IImsupp_typ_def by simp
+lemma IImsupp_type_TVr[simp]: "IImsupp_type TVr = {}"
+  unfolding IImsupp_type_def by simp
 
-lemma SSupp_typ_fun_upd_le: "SSupp_typ (f(X := T)) \<subseteq> insert X (SSupp_typ f)"
-  unfolding SSupp_typ_def by auto
+lemma SSupp_type_fun_upd_le: "SSupp_type (f(X := T)) \<subseteq> insert X (SSupp_type f)"
+  unfolding SSupp_type_def by auto
 
-lemma SSupp_typ_fun_upd_bound[simp]: "|SSupp_typ (f(X := T))| <o |UNIV :: 'a::var set| \<longleftrightarrow> |SSupp_typ f| <o |UNIV :: 'a set|"
+lemma SSupp_type_fun_upd_bound[simp]: "|SSupp_type (f(X := T))| <o |UNIV :: 'a::var set| \<longleftrightarrow> |SSupp_type f| <o |UNIV :: 'a set|"
   apply safe
-   apply (metis SSupp_typ_fun_upd_le card_of_mono1 fun_upd_idem_iff fun_upd_upd infinite_UNIV insert_bound ordLeq_ordLess_trans)
-  apply (meson SSupp_typ_fun_upd_le card_of_mono1 infinite_UNIV insert_bound ordLeq_ordLess_trans)
+   apply (metis SSupp_type_fun_upd_le card_of_mono1 fun_upd_idem_iff fun_upd_upd infinite_UNIV insert_bound ordLeq_ordLess_trans)
+  apply (meson SSupp_type_fun_upd_le card_of_mono1 infinite_UNIV insert_bound ordLeq_ordLess_trans)
   done
 
-lemma permute_typ_eq_tvsubst_typ_TyVar:
+lemma permute_type_eq_substT_TVr:
 assumes "bij (\<sigma>::'a\<Rightarrow>'a)" "|supp \<sigma>| <o |UNIV::'a::var set|"
-shows "permute_typ \<sigma> = tvsubst_typ (TyVar o \<sigma>)"
+shows "permute_type \<sigma> = substT (TVr o \<sigma>)"
 proof
   fix T
-  show "permute_typ \<sigma> T = tvsubst_typ (TyVar o \<sigma>) T"
-  proof (binder_induction T avoiding: "IImsupp_typ (TyVar \<circ> \<sigma>)" T rule: typ.strong_induct)
+  show "permute_type \<sigma> T = substT (TVr o \<sigma>) T"
+  proof (binder_induction T avoiding: "IImsupp_type (TVr \<circ> \<sigma>)" T rule: type.strong_induct)
     case Bound
     then show ?case using assms
-      by (auto simp: IImsupp_typ_def infinite_UNIV intro!: typ.Un_bound typ.UN_bound typ.SSupp_comp_bound)
+      by (auto simp: IImsupp_type_def infinite_UNIV intro!: type.Un_bound type.UN_bound type.SSupp_comp_bound)
   next
-    case (Forall X T1 T2)
+    case (All X T1 T2)
     then show ?case
-      by (subst typ.subst)
-        (auto simp: assms infinite_UNIV SSupp_typ_TyVar_comp IImsupp_typ_TyVar_comp
-          typ_inject id_on_def FVars_tvsubst_typ supp_inv_bound imsupp_def not_in_supp_alt
+      by (subst type.subst)
+        (auto simp: assms infinite_UNIV SSupp_type_TVr_comp IImsupp_type_TVr_comp
+          type_inject id_on_def FVars_substT supp_inv_bound imsupp_def not_in_supp_alt
           intro!: exI[of _ id])
-  qed (auto simp: assms infinite_UNIV SSupp_typ_TyVar_comp intro: lfset.map_cong)
+  qed (auto simp: assms infinite_UNIV SSupp_type_TVr_comp intro: lfset.map_cong)
 qed
 
-lemma permute_typ_eq_tvsubst_typ_TyVar':
-"bij (\<sigma>::'a::var\<Rightarrow>'a) \<Longrightarrow> |supp \<sigma>| <o |UNIV::'a set| \<Longrightarrow> permute_typ \<sigma> T = tvsubst_typ (TyVar o \<sigma>) T"
-  using permute_typ_eq_tvsubst_typ_TyVar by metis
+lemma permute_type_eq_substT_TVr':
+"bij (\<sigma>::'a::var\<Rightarrow>'a) \<Longrightarrow> |supp \<sigma>| <o |UNIV::'a set| \<Longrightarrow> permute_type \<sigma> T = substT (TVr o \<sigma>) T"
+  using permute_type_eq_substT_TVr by metis
 
-lemma IImsupp_typ_bound:
-  fixes f ::"'a::var \<Rightarrow> 'a typ"
-  assumes "|SSupp_typ f| <o |UNIV::'a set|"
-  shows "|IImsupp_typ f| <o |UNIV::'a set|"
-  unfolding IImsupp_typ_def using assms
-  by (simp add: lfset.UN_bound lfset.Un_bound typ.set_bd_UNIV)
+lemma IImsupp_type_bound:
+  fixes f ::"'a::var \<Rightarrow> 'a type"
+  assumes "|SSupp_type f| <o |UNIV::'a set|"
+  shows "|IImsupp_type f| <o |UNIV::'a set|"
+  unfolding IImsupp_type_def using assms
+  by (simp add: lfset.UN_bound lfset.Un_bound type.set_bd_UNIV)
 
-lemma SSupp_typ_tvsubst_typ:
-  fixes f g ::"'a::var \<Rightarrow> 'a typ"
-  assumes "|SSupp_typ f| <o |UNIV::'a set|"
-  shows "SSupp_typ (tvsubst_typ f \<circ> g) \<subseteq> SSupp_typ f \<union> SSupp_typ g"
-  using assms by (auto simp: SSupp_typ_def)
+lemma SSupp_type_substT:
+  fixes f g ::"'a::var \<Rightarrow> 'a type"
+  assumes "|SSupp_type f| <o |UNIV::'a set|"
+  shows "SSupp_type (substT f \<circ> g) \<subseteq> SSupp_type f \<union> SSupp_type g"
+  using assms by (auto simp: SSupp_type_def)
 
-lemma IImsupp_typ_tvsubst_typ:
-  fixes f g ::"'a::var \<Rightarrow> 'a typ"
-  assumes "|SSupp_typ f| <o |UNIV::'a set|"
-  shows "IImsupp_typ (tvsubst_typ f \<circ> g) \<subseteq> IImsupp_typ f \<union> IImsupp_typ g"
-  using assms using SSupp_typ_tvsubst_typ[of f g]
-  apply (auto simp: IImsupp_typ_def FVars_tvsubst_typ)
-  by (metis (mono_tags, lifting) SSupp_typ_def Un_iff mem_Collect_eq singletonD sup.orderE typ.FVars_VVr)
+lemma IImsupp_type_substT:
+  fixes f g ::"'a::var \<Rightarrow> 'a type"
+  assumes "|SSupp_type f| <o |UNIV::'a set|"
+  shows "IImsupp_type (substT f \<circ> g) \<subseteq> IImsupp_type f \<union> IImsupp_type g"
+  using assms using SSupp_type_substT[of f g]
+  apply (auto simp: IImsupp_type_def FVars_substT)
+  by (metis (mono_tags, lifting) SSupp_type_def Un_iff mem_Collect_eq singletonD sup.orderE type.FVars_VVr)
 
-lemma SSupp_typ_tvsubst_typ_bound:
-  fixes f g ::"'a::var \<Rightarrow> 'a typ"
-  assumes "|SSupp_typ f| <o |UNIV::'a set|"
-  assumes "|SSupp_typ g| <o |UNIV::'a set|"
-  shows "|SSupp_typ (tvsubst_typ f \<circ> g)| <o |UNIV :: 'a set|"
-  using SSupp_typ_tvsubst_typ[of f g] assms
+lemma SSupp_type_substT_bound:
+  fixes f g ::"'a::var \<Rightarrow> 'a type"
+  assumes "|SSupp_type f| <o |UNIV::'a set|"
+  assumes "|SSupp_type g| <o |UNIV::'a set|"
+  shows "|SSupp_type (substT f \<circ> g)| <o |UNIV :: 'a set|"
+  using SSupp_type_substT[of f g] assms
   by (simp add: card_of_subset_bound lfset.Un_bound)
 
-lemma tvsubst_typ_TyVar[simp]: "tvsubst_typ TyVar T = T"
-  by (binder_induction T avoiding: T rule: typ.strong_induct)
-    (auto simp: IImsupp_typ_def intro!: trans[OF lfset.map_cong lfset.map_id])
+lemma substT_TVr[simp]: "substT TVr T = T"
+  by (binder_induction T avoiding: T rule: type.strong_induct)
+    (auto simp: IImsupp_type_def intro!: trans[OF lfset.map_cong lfset.map_id])
 
-lemma tvsubst_typ_comp:
-  fixes f g ::"'a::var \<Rightarrow> 'a typ"
-  assumes "|SSupp_typ f| <o |UNIV::'a set|"
-  assumes "|SSupp_typ g| <o |UNIV::'a set|"
-  shows "tvsubst_typ g (tvsubst_typ f T) = tvsubst_typ (tvsubst_typ g o f) T"
-proof (binder_induction T avoiding: "IImsupp_typ f" "IImsupp_typ g" T rule: typ.strong_induct)
-  case (Forall X T U)
+lemma substT_comp:
+  fixes f g ::"'a::var \<Rightarrow> 'a type"
+  assumes "|SSupp_type f| <o |UNIV::'a set|"
+  assumes "|SSupp_type g| <o |UNIV::'a set|"
+  shows "substT g (substT f T) = substT (substT g o f) T"
+proof (binder_induction T avoiding: "IImsupp_type f" "IImsupp_type g" T rule: type.strong_induct)
+  case (All X T U)
   then show ?case
-    apply (subst typ.subst; simp add: assms)
-    apply (subst typ.subst; (simp add: assms FVars_tvsubst_typ)?)
-    apply (metis VVr_eq_TyVar singletonD typ.in_IImsupp typ.set(1))
-    apply (subst typ.subst; (simp add: assms SSupp_typ_tvsubst_typ_bound)?)
-    using IImsupp_typ_tvsubst_typ assms(2) by blast
-qed (auto simp: assms SSupp_typ_tvsubst_typ_bound IImsupp_typ_bound lfset.map_comp intro: lfset.map_cong)
+    apply (subst type.subst; simp add: assms)
+    apply (subst type.subst; (simp add: assms FVars_substT)?)
+    apply (metis VVr_eq_TVr singletonD type.in_IImsupp type.set(1))
+    apply (subst type.subst; (simp add: assms SSupp_type_substT_bound)?)
+    using IImsupp_type_substT assms(2) by blast
+qed (auto simp: assms SSupp_type_substT_bound IImsupp_type_bound lfset.map_comp intro: lfset.map_cong)
 
-lemma tvsubst_typ_cong:
-  fixes f g ::"'a::var \<Rightarrow> 'a typ"
-  assumes "|SSupp_typ f| <o |UNIV::'a set|"
-  assumes "|SSupp_typ g| <o |UNIV::'a set|"
-  shows "(\<forall>x \<in> FVars_typ T. f x = g x) \<Longrightarrow> tvsubst_typ f T = tvsubst_typ g T"
-proof (binder_induction T avoiding: "IImsupp_typ f" "IImsupp_typ g" T rule: typ.strong_induct)
-  case (Forall X T U)
+lemma substT_cong:
+  fixes f g ::"'a::var \<Rightarrow> 'a type"
+  assumes "|SSupp_type f| <o |UNIV::'a set|"
+  assumes "|SSupp_type g| <o |UNIV::'a set|"
+  shows "(\<forall>x \<in> TFV T. f x = g x) \<Longrightarrow> substT f T = substT g T"
+proof (binder_induction T avoiding: "IImsupp_type f" "IImsupp_type g" T rule: type.strong_induct)
+  case (All X T U)
   then show ?case
-    apply (subst (1 2) typ.subst; simp add: assms)
-    by (metis (mono_tags, lifting) DiffI IImsupp_typ_def SSupp_typ_def Un_iff mem_Collect_eq singletonD)
-qed (auto simp: assms IImsupp_typ_bound intro: lfset.map_cong)
+    apply (subst (1 2) type.subst; simp add: assms)
+    by (metis (mono_tags, lifting) DiffI IImsupp_type_def SSupp_type_def Un_iff mem_Collect_eq singletonD)
+qed (auto simp: assms IImsupp_type_bound intro: lfset.map_cong)
 
-lemma vvsubst_typ_tvsubst_typ:
-  fixes T :: "'tv :: var typ"
+lemma vvsubst_type_substT:
+  fixes T :: "'tv :: var type"
   assumes "|supp \<tau>| <o |UNIV :: 'tv ::var set|"
-  shows "vvsubst_typ \<tau> T = tvsubst_typ (TyVar o \<tau>) T"
-  by (binder_induction T avoiding: T "imsupp \<tau>" rule: typ.strong_induct)
-    (auto simp: SSupp_typ_TyVar_comp IImsupp_typ_TyVar_comp
+  shows "vvsubst_type \<tau> T = substT (TVr o \<tau>) T"
+  by (binder_induction T avoiding: T "imsupp \<tau>" rule: type.strong_induct)
+    (auto simp: SSupp_type_TVr_comp IImsupp_type_TVr_comp
       assms imsupp_supp_bound infinite_UNIV intro: lfset.map_cong)
 
-lemma finite_FVars_typ[simp]:"finite (FVars_typ T)"
+lemma finite_TFV[simp]:"finite (TFV T)"
   by (induct T) auto
 
 end
