thys/POPLmark/POPLmark_1B.thy
@@ -5,8 +5,8 @@ begin
 (********************* Actual formalization ************************)
 
 lemma ty_refl: "\<lbrakk> \<turnstile> \<Gamma> ok ; T closed_in \<Gamma> \<rbrakk> \<Longrightarrow> \<Gamma> \<turnstile> T <: T"
-proof (binder_induction T arbitrary: \<Gamma> avoiding: "dom \<Gamma>" rule: typ.strong_induct)
-  case (TyVar x \<Gamma>)
+proof (binder_induction T arbitrary: \<Gamma> avoiding: "dom \<Gamma>" rule: type.strong_induct)
+  case (TVr x \<Gamma>)
   then show ?case by blast
 next
   case (TRec x \<Gamma>)
@@ -97,22 +97,22 @@ qed auto
 lemma SA_AllE1[consumes 2, case_names SA_Trans_TVar SA_All]:
   assumes "\<Gamma> \<turnstile> \<forall>X<:S\<^sub>1. S\<^sub>2 <: T" "X \<notin> dom \<Gamma>"
     and Top: "\<And>\<Gamma>. \<lbrakk> \<turnstile> \<Gamma> ok ; \<forall>X<:S\<^sub>1. S\<^sub>2 closed_in \<Gamma> \<rbrakk> \<Longrightarrow> R \<Gamma> (\<forall>X<:S\<^sub>1. S\<^sub>2) Top"
-    and Forall: "\<And>\<Gamma> T\<^sub>1 T\<^sub>2. \<lbrakk> \<Gamma> \<turnstile> T\<^sub>1 <: S\<^sub>1 ; \<Gamma> \<^bold>, X<:T\<^sub>1 \<turnstile> S\<^sub>2 <: T\<^sub>2 \<rbrakk> \<Longrightarrow> R \<Gamma> (\<forall>X<:S\<^sub>1. S\<^sub>2) (\<forall>X<:T\<^sub>1 . T\<^sub>2)"
+    and All: "\<And>\<Gamma> T\<^sub>1 T\<^sub>2. \<lbrakk> \<Gamma> \<turnstile> T\<^sub>1 <: S\<^sub>1 ; \<Gamma> \<^bold>, X<:T\<^sub>1 \<turnstile> S\<^sub>2 <: T\<^sub>2 \<rbrakk> \<Longrightarrow> R \<Gamma> (\<forall>X<:S\<^sub>1. S\<^sub>2) (\<forall>X<:T\<^sub>1 . T\<^sub>2)"
   shows "R \<Gamma> (\<forall>X<:S\<^sub>1. S\<^sub>2) T"
 using assms(1,2) proof (binder_induction \<Gamma> "\<forall>X<:S\<^sub>1. S\<^sub>2" T avoiding: \<Gamma> "\<forall>X<:S\<^sub>1. S\<^sub>2" T rule: ty.strong_induct)
   case (SA_All \<Gamma> T\<^sub>1 R\<^sub>1 Y R\<^sub>2 T\<^sub>2)
-  have 1: "\<forall>Y<:T\<^sub>1 . T\<^sub>2 = \<forall>X<:T\<^sub>1. permute_typ (X \<leftrightarrow> Y) T\<^sub>2"
-    unfolding typ.inject
+  have 1: "\<forall>Y<:T\<^sub>1 . T\<^sub>2 = \<forall>X<:T\<^sub>1. permute_type (X \<leftrightarrow> Y) T\<^sub>2"
+    unfolding type.inject
     using SA_All(10,7) well_scoped(2) by (fastforce simp: swap_sym)
-  have fresh: "X \<notin> FVars_typ T\<^sub>1"
+  have fresh: "X \<notin> TFV T\<^sub>1"
     by (meson SA_All(5,10) in_mono well_scoped(1))
-  have same: "R\<^sub>1 = S\<^sub>1" using SA_All(9) typ_inject by blast
-  have x: "\<forall>Y<:S\<^sub>1. R\<^sub>2 = \<forall>X<:S\<^sub>1. permute_typ (X \<leftrightarrow> Y) R\<^sub>2"
-    unfolding typ.inject
+  have same: "R\<^sub>1 = S\<^sub>1" using SA_All(9) type_inject by blast
+  have x: "\<forall>Y<:S\<^sub>1. R\<^sub>2 = \<forall>X<:S\<^sub>1. permute_type (X \<leftrightarrow> Y) R\<^sub>2"
+    unfolding type.inject
     apply (auto simp: swap_sym)
-    using SA_All.hyps(9) typ.inject(3) by blast
+    using SA_All.hyps(9) type.inject(3) by blast
   show ?case unfolding 1
-    apply (rule Forall)
+    apply (rule All)
     using same SA_All(5) apply simp
     apply (rule iffD2[OF arg_cong3[OF _ _ refl, of _ _ _ _ ty], rotated -1])
       apply (rule ty.equiv)
@@ -127,32 +127,32 @@ using assms(1,2) proof (binder_induction \<Gamma> "\<forall>X<:S\<^sub>1. S\<^su
       apply simp
     using fresh SA_All(4) apply simp
     using x SA_All(9) unfolding same
-    by (metis typ.inject(3))
+    by (metis type.inject(3))
 qed (auto simp: Top)
 
 lemma SA_AllE2[consumes 2, case_names SA_Trans_TVar SA_All]:
   assumes "\<Gamma> \<turnstile> S <: \<forall>X<:T\<^sub>1. T\<^sub>2" "X \<notin> dom \<Gamma>"
-    and TyVar: "\<And>\<Gamma> x U. \<lbrakk> x<:U \<in> \<Gamma> ; \<Gamma> \<turnstile> U <: \<forall> X <: T\<^sub>1 . T\<^sub>2 ; R \<Gamma> U (\<forall>X<:T\<^sub>1. T\<^sub>2) \<rbrakk> \<Longrightarrow> R \<Gamma> (TyVar x) (\<forall> X <: T\<^sub>1 . T\<^sub>2)"
-    and Forall: "\<And>\<Gamma> S\<^sub>1 S\<^sub>2. \<lbrakk> \<Gamma> \<turnstile> T\<^sub>1 <: S\<^sub>1 ; \<Gamma> \<^bold>, X<:T\<^sub>1 \<turnstile> S\<^sub>2 <: T\<^sub>2 \<rbrakk> \<Longrightarrow> R \<Gamma> (\<forall>X<:S\<^sub>1. S\<^sub>2) (\<forall> X <: T\<^sub>1 . T\<^sub>2)"
+    and TVr: "\<And>\<Gamma> x U. \<lbrakk> x<:U \<in> \<Gamma> ; \<Gamma> \<turnstile> U <: \<forall> X <: T\<^sub>1 . T\<^sub>2 ; R \<Gamma> U (\<forall>X<:T\<^sub>1. T\<^sub>2) \<rbrakk> \<Longrightarrow> R \<Gamma> (TVr x) (\<forall> X <: T\<^sub>1 . T\<^sub>2)"
+    and All: "\<And>\<Gamma> S\<^sub>1 S\<^sub>2. \<lbrakk> \<Gamma> \<turnstile> T\<^sub>1 <: S\<^sub>1 ; \<Gamma> \<^bold>, X<:T\<^sub>1 \<turnstile> S\<^sub>2 <: T\<^sub>2 \<rbrakk> \<Longrightarrow> R \<Gamma> (\<forall>X<:S\<^sub>1. S\<^sub>2) (\<forall> X <: T\<^sub>1 . T\<^sub>2)"
   shows "R \<Gamma> S (\<forall>X<:T\<^sub>1. T\<^sub>2)"
 using assms(1,2) proof (binder_induction \<Gamma> S "\<forall>X<:T\<^sub>1. T\<^sub>2" avoiding: \<Gamma> S "\<forall>X<:T\<^sub>1. T\<^sub>2" rule: ty.strong_induct)
   case (SA_All \<Gamma> R\<^sub>1 S\<^sub>1 Y S\<^sub>2 R\<^sub>2)
-  have 1: "\<forall>Y<:S\<^sub>1. S\<^sub>2 = \<forall>X<:S\<^sub>1. permute_typ (Y \<leftrightarrow> X) S\<^sub>2"
-    unfolding typ.inject
+  have 1: "\<forall>Y<:S\<^sub>1. S\<^sub>2 = \<forall>X<:S\<^sub>1. permute_type (Y \<leftrightarrow> X) S\<^sub>2"
+    unfolding type.inject
     using SA_All.hyps(10,7) well_scoped(1) by fastforce
   have fresh: "X \<notin> dom \<Gamma>" "Y \<notin> dom \<Gamma>"
     using SA_All(10) apply blast
     by (metis SA_All(7) fst_conv wf_ConsE wf_context)
-  have fresh2: "X \<notin> FVars_typ T\<^sub>1" "Y \<notin> FVars_typ T\<^sub>1"
-     apply (metis SA_All(5,9) in_mono fresh(1) typ_inject well_scoped(1))
-    by (metis SA_All(5,9) in_mono fresh(2) typ_inject well_scoped(1))
-  have same: "R\<^sub>1 = T\<^sub>1" using SA_All(9) typ_inject by blast
-  have x: "\<forall>Y<:T\<^sub>1 . R\<^sub>2 = \<forall>X<:T\<^sub>1. permute_typ (Y \<leftrightarrow> X) R\<^sub>2"
-    unfolding typ.inject apply auto
-    using SA_All.hyps(9) typ.inject(3) by blast
+  have fresh2: "X \<notin> TFV T\<^sub>1" "Y \<notin> TFV T\<^sub>1"
+     apply (metis SA_All(5,9) in_mono fresh(1) type_inject well_scoped(1))
+    by (metis SA_All(5,9) in_mono fresh(2) type_inject well_scoped(1))
+  have same: "R\<^sub>1 = T\<^sub>1" using SA_All(9) type_inject by blast
+  have x: "\<forall>Y<:T\<^sub>1 . R\<^sub>2 = \<forall>X<:T\<^sub>1. permute_type (Y \<leftrightarrow> X) R\<^sub>2"
+    unfolding type.inject apply auto
+    using SA_All.hyps(9) type.inject(3) by blast
   show ?case unfolding 1
-    apply (rule Forall)
-     apply (metis SA_All(5,9) typ_inject)
+    apply (rule All)
+     apply (metis SA_All(5,9) type_inject)
     apply (rule iffD2[OF arg_cong3[OF _ refl, of _ _ _ _ ty], rotated -1])
       apply (rule ty.equiv)
        apply (rule bij_swap supp_swap_bound infinite_UNIV)+
@@ -166,8 +166,8 @@ using assms(1,2) proof (binder_induction \<Gamma> S "\<forall>X<:T\<^sub>1. T\<^
       apply simp
     using fresh2 unfolding same apply simp
     using SA_All(9) x unfolding same
-    using Forall_swapD by blast
-qed (auto simp: TyVar)
+    using All_swapD by blast
+qed (auto simp: TVr)
 
 lemma ty_transitivity : "\<lbrakk> \<Gamma> \<turnstile> S <: Q ; \<Gamma> \<turnstile> Q <: T \<rbrakk> \<Longrightarrow> \<Gamma> \<turnstile> S <: T"
   and ty_narrowing : "\<lbrakk> \<Gamma> \<^bold>, X <: Q\<^bold>, \<Delta> \<turnstile> M <: N ; \<Gamma> \<turnstile> R <: Q \<rbrakk> \<Longrightarrow> \<Gamma> \<^bold>, X <: R\<^bold>, \<Delta> \<turnstile> M <: N"
@@ -175,25 +175,25 @@ proof -
   have
     ty_trans: "\<lbrakk> \<Gamma> \<turnstile> S <: Q ; \<Gamma> \<turnstile> Q <: T \<rbrakk> \<Longrightarrow> \<Gamma> \<turnstile> S <: T"
   and ty_narrow: "\<lbrakk> (\<Gamma> \<^bold>, X <: Q)\<^bold>, \<Delta> \<turnstile> M <: N ; \<Gamma> \<turnstile> R <: Q ; \<turnstile> \<Gamma> \<^bold>, X <: R\<^bold>, \<Delta> ok ; M closed_in (\<Gamma> \<^bold>, X <: R\<^bold>, \<Delta>) ; N closed_in (\<Gamma> \<^bold>, X <: R\<^bold>, \<Delta>) \<rbrakk> \<Longrightarrow> (\<Gamma> \<^bold>, X <: R)\<^bold>, \<Delta> \<turnstile> M <: N"
-  proof (binder_induction Q arbitrary: \<Gamma> \<Delta> S T M N X R avoiding: X "dom \<Gamma>" "dom \<Delta>" rule: typ.strong_induct)
-    case (TyVar Y \<Gamma> \<Delta> S T M N X R)
+  proof (binder_induction Q arbitrary: \<Gamma> \<Delta> S T M N X R avoiding: X "dom \<Gamma>" "dom \<Delta>" rule: type.strong_induct)
+    case (TVr Y \<Gamma> \<Delta> S T M N X R)
     {
       fix \<Gamma> S T
-      show ty_trans: "\<Gamma> \<turnstile> S <: TyVar Y \<Longrightarrow> \<Gamma> \<turnstile> TyVar Y <: T \<Longrightarrow> \<Gamma> \<turnstile> S <: T"
-        by (induction \<Gamma> S "TyVar Y" rule: ty.induct) auto
+      show ty_trans: "\<Gamma> \<turnstile> S <: TVr Y \<Longrightarrow> \<Gamma> \<turnstile> TVr Y <: T \<Longrightarrow> \<Gamma> \<turnstile> S <: T"
+        by (induction \<Gamma> S "TVr Y" rule: ty.induct) auto
     } note ty_trans = this
     {
       case 2
       then show ?case
-      proof (binder_induction "\<Gamma> \<^bold>, X <: TyVar Y\<^bold>, \<Delta>" M N arbitrary: \<Delta> avoiding: X "dom \<Gamma>" "dom \<Delta>" rule: ty.strong_induct)
+      proof (binder_induction "\<Gamma> \<^bold>, X <: TVr Y\<^bold>, \<Delta>" M N arbitrary: \<Delta> avoiding: X "dom \<Gamma>" "dom \<Delta>" rule: ty.strong_induct)
         case (SA_Trans_TVar Z U T \<Delta>')
         show ?case
         proof (cases "X = Z")
           case True
-          then have u: "U = TyVar Y" using SA_Trans_TVar(1,2) context_determ wf_context by blast
-          have "TyVar Y closed_in \<Gamma> \<^bold>, Z <: R\<^bold>, \<Delta>'" using SA_Trans_TVar(2) True u well_scoped(1) by fastforce
-          then have "\<Gamma> \<^bold>, Z <: R \<^bold>, \<Delta>' \<turnstile> TyVar Y <: T" using SA_Trans_TVar True u by auto
-          moreover have "\<Gamma> \<^bold>, Z <: R\<^bold>, \<Delta>' \<turnstile> R <: TyVar Y" using ty_weakening[OF ty_weakening_extend[OF SA_Trans_TVar(4)]]
+          then have u: "U = TVr Y" using SA_Trans_TVar(1,2) context_determ wf_context by blast
+          have "TVr Y closed_in \<Gamma> \<^bold>, Z <: R\<^bold>, \<Delta>'" using SA_Trans_TVar(2) True u well_scoped(1) by fastforce
+          then have "\<Gamma> \<^bold>, Z <: R \<^bold>, \<Delta>' \<turnstile> TVr Y <: T" using SA_Trans_TVar True u by auto
+          moreover have "\<Gamma> \<^bold>, Z <: R\<^bold>, \<Delta>' \<turnstile> R <: TVr Y" using ty_weakening[OF ty_weakening_extend[OF SA_Trans_TVar(4)]]
             by (metis SA_Trans_TVar(5) True wf_ConsE wf_concatD)
           ultimately have "\<Gamma> \<^bold>, Z <: R \<^bold>, \<Delta>' \<turnstile> R <: T" using ty_trans by blast
           then show ?thesis unfolding True u using ty.SA_Trans_TVar by auto
@@ -218,7 +218,7 @@ proof -
       next
         case (SA_TRec X Y \<Delta>')
         then show ?case
-          by (smt (verit, del_insts) SA_TRecER ty.SA_TRec ty_refl typ.distinct(4) well_scoped(2))
+          by (smt (verit, del_insts) SA_TRecER ty.SA_TRec ty_refl type.distinct(4) well_scoped(2))
       qed (rule context_set_bd_UNIV | blast)+
     }
   next
@@ -258,11 +258,11 @@ proof -
       next
         case (SA_TRec X Y \<Delta>')
         then show ?case
-          by (smt (verit) SA_TRecER ty.SA_TRec ty_refl typ.distinct(17) well_scoped(2))
+          by (smt (verit) SA_TRecER ty.SA_TRec ty_refl type.distinct(17) well_scoped(2))
       qed (rule context_set_bd_UNIV | blast)+
     }
   next
-    case (Fun Q\<^sub>1 Q\<^sub>2 \<Gamma> \<Delta> S T M N X R)
+    case (Arr Q\<^sub>1 Q\<^sub>2 \<Gamma> \<Delta> S T M N X R)
     {
       fix \<Gamma> S T
       assume "\<Gamma> \<turnstile> S <: Q\<^sub>1 \<rightarrow> Q\<^sub>2" "\<Gamma> \<turnstile> Q\<^sub>1 \<rightarrow> Q\<^sub>2 <: T"
@@ -275,7 +275,7 @@ proof -
           then show ?thesis by (meson left(1,3) ty.SA_Arrow ty.SA_Top well_scoped(1))
         next
           case right: (SA_Arrow U\<^sub>1 R\<^sub>1 R\<^sub>2 U\<^sub>2)
-          then show ?thesis using left by (metis Fun(1,3) SA_Arrow typ.inject)
+          then show ?thesis using left by (metis Arr(1,3) SA_Arrow type.inject)
         qed auto
       qed auto
     } note ty_trans = this
@@ -315,11 +315,11 @@ proof -
       next
         case (SA_TRec X Y \<Delta>')
         then show ?case
-          by (smt (verit, ccfv_threshold) SA_TRecER ty.SA_TRec ty_refl typ.distinct(17) well_scoped(2))
+          by (smt (verit, ccfv_threshold) SA_TRecER ty.SA_TRec ty_refl type.distinct(17) well_scoped(2))
       qed (rule context_set_bd_UNIV | blast)+
     }
   next
-    case (Forall X Q\<^sub>1 Q\<^sub>2 \<Gamma> \<Delta> S T M N Y R)
+    case (All X Q\<^sub>1 Q\<^sub>2 \<Gamma> \<Delta> S T M N Y R)
     have ty_trans: "\<And>\<Gamma> S T. X \<notin> dom \<Gamma> \<Longrightarrow> \<Gamma> \<turnstile> S <: \<forall>X<:Q\<^sub>1. Q\<^sub>2 \<Longrightarrow> \<Gamma> \<turnstile> \<forall>X<:Q\<^sub>1. Q\<^sub>2 <: T \<Longrightarrow> \<Gamma> \<turnstile> S <: T"
     proof -
       fix \<Gamma> S T
@@ -333,20 +333,20 @@ proof -
           then show ?case by (meson SA_Top ty.SA_All well_scoped(1))
         next
           case (SA_All \<Gamma> T\<^sub>1 T\<^sub>2)
-          have 1: "\<Gamma> \<turnstile> T\<^sub>1 <: S\<^sub>1" by (rule Forall(4)[OF SA_All(1,3)])
-          have "\<Gamma> \<^bold>, X <: T\<^sub>1 \<turnstile> S\<^sub>2 <: Q\<^sub>2" using Forall(5)[of \<emptyset> X \<Gamma> S\<^sub>2 Q\<^sub>2, OF _ SA_All(1)] SA_All(4)
+          have 1: "\<Gamma> \<turnstile> T\<^sub>1 <: S\<^sub>1" by (rule All(4)[OF SA_All(1,3)])
+          have "\<Gamma> \<^bold>, X <: T\<^sub>1 \<turnstile> S\<^sub>2 <: Q\<^sub>2" using All(5)[of \<emptyset> X \<Gamma> S\<^sub>2 Q\<^sub>2, OF _ SA_All(1)] SA_All(4)
             by (metis (mono_tags, lifting) SA_All(2) append.left_neutral fst_conv image_insert list.simps(15) well_scoped(1) wf_context)
-          then have "\<Gamma> \<^bold>, X <: T\<^sub>1 \<turnstile> S\<^sub>2 <: T\<^sub>2" by (rule Forall(6)[OF _ SA_All(2)])
+          then have "\<Gamma> \<^bold>, X <: T\<^sub>1 \<turnstile> S\<^sub>2 <: T\<^sub>2" by (rule All(6)[OF _ SA_All(2)])
           then show ?case using 1 by blast
         qed
       qed auto
     qed
     {
       case 1
-      then show ?case using ty_trans Forall(2) by blast
+      then show ?case using ty_trans All(2) by blast
     next
       case 2
-      then show ?case using Forall(1-3)
+      then show ?case using All(1-3)
       proof (binder_induction "\<Gamma> \<^bold>, Y <: (\<forall>X<:Q\<^sub>1. Q\<^sub>2) \<^bold>, \<Delta>" M N arbitrary: \<Delta> avoiding: X Y "dom \<Gamma>" "dom \<Delta>" rule: ty.strong_induct)
         case (SA_Trans_TVar Z U T \<Delta>')
         then show ?case
@@ -386,7 +386,7 @@ proof -
       next
         case (SA_TRec X Y \<Delta>')
         then show ?case
-          by (smt (verit) SA_TRecER ty.SA_TRec ty_refl typ.distinct(17) well_scoped(2))
+          by (smt (verit) SA_TRecER ty.SA_TRec ty_refl type.distinct(17) well_scoped(2))
       qed (rule context_set_bd_UNIV | blast)+
     }
   next
@@ -435,7 +435,7 @@ proof -
       next
         case (SA_TRec X Y)
         then show ?case
-          by (smt (verit, ccfv_threshold) SA_TRecER ty.SA_TRec ty_refl typ.distinct(17) well_scoped(2))
+          by (smt (verit, ccfv_threshold) SA_TRecER ty.SA_TRec ty_refl type.distinct(17) well_scoped(2))
       qed blast+
     }
   qed simp_all
@@ -477,13 +477,13 @@ proof -
 qed
 
 theorem ty_transitivity2: "\<lbrakk> \<Gamma> \<turnstile> S <: Q ; \<Gamma> \<turnstile> Q <: T \<rbrakk> \<Longrightarrow> \<Gamma> \<turnstile> S <: T"
-proof (binder_induction Q arbitrary: \<Gamma> S T avoiding: "dom \<Gamma>" rule: typ.strong_induct)
-  case (TyVar x \<Gamma> S T)
+proof (binder_induction Q arbitrary: \<Gamma> S T avoiding: "dom \<Gamma>" rule: type.strong_induct)
+  case (TVr x \<Gamma> S T)
   then show ?case
-    by (induction \<Gamma> S "TyVar x") auto
+    by (induction \<Gamma> S "TVr x") auto
 next
-  case (Fun x1 x2 \<Gamma> S T)
-  from Fun(4,3) show ?case
+  case (Arr x1 x2 \<Gamma> S T)
+  from Arr(4,3) show ?case
   proof (induction \<Gamma> "x1 \<rightarrow> x2" T)
     case (SA_Top \<Gamma>)
     then show ?case using well_scoped by blast
@@ -494,13 +494,13 @@ next
       case (SA_Arrow \<Gamma> U\<^sub>1 R\<^sub>1 R\<^sub>2 U\<^sub>2)
       show ?case
         apply (rule ty.SA_Arrow)
-         apply (metis Fun(1) SA_Arrow(1,5,6,8) typ.inject(2))
-        by (metis Fun(2) SA_Arrow(3,5,7,8) typ.inject(2))
+         apply (metis Arr(1) SA_Arrow(1,5,6,8) type.inject(2))
+        by (metis Arr(2) SA_Arrow(3,5,7,8) type.inject(2))
     qed auto
   qed auto
 next
-  case (Forall X Q\<^sub>1 Q\<^sub>2 \<Gamma> S T)
-  from Forall(4,1,5,1) show ?case
+  case (All X Q\<^sub>1 Q\<^sub>2 \<Gamma> S T)
+  from All(4,1,5,1) show ?case
   proof (induction rule: SA_AllE2)
     case outer: (SA_All \<Gamma> S\<^sub>1 S\<^sub>2)
     from outer(3,4,1,2,4) show ?case
@@ -510,9 +510,9 @@ next
     next
       case (SA_All \<Gamma> T\<^sub>1 T\<^sub>2)
       then have "\<Gamma> \<^bold>, X <: T\<^sub>1 \<turnstile> S\<^sub>2 <: Q\<^sub>2"
-        using ty_narrowing_aux[where \<Delta>="[]", unfolded append.simps] Forall(2) by blast
-      then have "\<Gamma> \<^bold>, X <: T\<^sub>1 \<turnstile> S\<^sub>2 <: T\<^sub>2" using Forall(3) SA_All(2) by blast
-      moreover have "\<Gamma> \<turnstile> T\<^sub>1 <: S\<^sub>1" by (rule Forall(2)[OF SA_All(1,3)])
+        using ty_narrowing_aux[where \<Delta>="[]", unfolded append.simps] All(2) by blast
+      then have "\<Gamma> \<^bold>, X <: T\<^sub>1 \<turnstile> S\<^sub>2 <: T\<^sub>2" using All(3) SA_All(2) by blast
+      moreover have "\<Gamma> \<turnstile> T\<^sub>1 <: S\<^sub>1" by (rule All(2)[OF SA_All(1,3)])
       ultimately show ?case by blast
     qed
   qed blast
